ulib/system.text.fsi
@@ -1,0 +1,2 @@
+module System.Text
+type StringBuilder
