lib/FStar.Constructive.fst
@@ -1,57 +1,61 @@
 module FStar.Constructive
-type cand p1 p2 =
+
+type cand (p1:Type) (p2:Type) : Type =
   | Conj : h1:p1 -> h2:p2 -> cand p1 p2
 
-type cor p1 p2 =
+type cor (p1:Type) (p2:Type) : Type =
   | IntroL : h:p1 -> cor p1 p2
   | IntroR : h:p2 -> cor p1 p2
 
-type cimp a b = a -> Tot b
+type cimp (a:Type) (b:Type) = a -> Tot b
 
-type ciff a b = cand (cimp a b) (cimp b a)
+type ciff (a:Type) (b:Type) = cand (cimp a b) (cimp b a)
 
-type cexists (#a:Type) (p:a -> Type) = 
+type cexists (#a:Type) (p:a -> Type) : Type =
   | ExIntro : x:a -> h:p x -> cexists p
 
-// val ex_intro_x : #a:Type -> #p:(a -> Type) -> projectee:cexists p -> Tot a
-// let ex_intro_x #a #p = function
-//   | ExIntro x _ -> x
+(* this currently fails because of ill-typed generated projector;
+   it's a strong elimination so we can't soundly allow that anyway *)
+(* type cexists_type (p:Type -> Type) : Type = *)
+(*   | ExTypeIntro : t:Type -> h:p t -> cexists_type p *)
 
-type ceq (#a:Type) x : a -> Type = 
+type ceq (#a:Type) (x:a) : a -> Type =
   | Refl : ceq #a x x
 
-type ceq_type a : Type -> Type =
+type ceq_type (a:Type) : Type -> Type =
   | ReflType : ceq_type a a
 
 val eq_ind : #a:Type -> x:a -> p:(a -> Type) -> f:p x -> y:a -> e:ceq x y -> Tot (p y)
-let eq_ind #a x p f y _ = f
+let eq_ind (a:Type) x (p:a -> Type) f y _ = f
 
 val ceq_eq : #a:Type -> #x:a -> #y:a -> h:(ceq x y) -> Lemma (x = y)
-let ceq_eq #a #x #y h = ()
+let ceq_eq (#a:Type) x y h = ()
 
 val ceq_congruence : #a:Type -> #b:Type -> #x:a -> #y:a -> ceq x y ->
                      f:(a -> GTot b) -> GTot (ceq (f x) (f y))
-let ceq_congruence #a #b #x #y h f = Refl #_ #(f x) //refuse to infer terms with non-Tot effect
+let ceq_congruence (a:Type) (b:Type) x y h f = Refl 
 
 val ceq_symm : #a:Type -> #x:a -> #y:a -> ceq x y -> Tot (ceq y x)
-let ceq_symm #a #x #y h = Refl
+let ceq_symm (a:Type) x y h = Refl
 
 val ceq_trans : #a:Type -> #x:a -> #y:a -> #z:a -> ceq x y -> ceq y z -> Tot (ceq x z)
-let ceq_trans #a #x #y #z hxy hyz = Refl
+let ceq_trans (a:Type) x y z hxy hyz = Refl
 
-type ctrue =
+type ctrue : Type =
   | I : ctrue
 
 (* hopefully this is an empty type *)
 type cfalse : Type =
 
-val cfalse_elim : #a:Type -> cfalse -> Tot a
-let cfalse_elim #a f = match f with 
-
-val false_elim2 : #a:Type -> cfalse -> Tot a
-let rec false_elim2 #a x = false_elim2 x
-
 val false_elim : #a:Type -> u:unit{false} -> Tot a
-let rec false_elim #a () = false_elim ()
+let rec false_elim (a:Type) () = false_elim ()
+
+assume val cfalse_elim : #a:Type -> cfalse -> Tot a
+(* This sholud work (see issue #70)
+E.g. in Coq: False_rect = fun (P:Type) (f:False) => match f return P with end
+let cfalse_elim f =
+  match f with
+  | _ -> 76 (* silly, fails type checking *)
+*)
 
 type cnot (p:Type) = cimp p cfalse
