lib/FStar.PredicateExtensionality.fst
@@ -6,11 +6,11 @@
 module FStar.PredicateExtensionality
 #set-options "--max_fuel 0 --initial_fuel 0 --initial_ifuel 0 --max_ifuel 0"
 
-let predicate (a:Type) = a -> Type
+kind Pred (a:Type) = a -> Type
 
-let peq (#a:Type) (p1:predicate a) (p2:predicate a) = forall x. p1 x <==> p2 x
+opaque logic type PEq : #a:Type -> (Pred a) -> (Pred a) -> Type =
+  (fun (a:Type) (p1:Pred a) (p2:Pred a) -> (forall x. p1 x <==> p2 x))
 
-assume val predicateExtensionality : a:Type -> p1:predicate a -> p2:predicate a ->
-  Lemma (requires True)
-	(ensures (peq #a p1 p2 <==> p1==p2))
-	[SMTPat (peq #a p1 p2)]
+assume PredicateExtensionality :
+    (forall (a:Type) (p1:Pred a) (p2:Pred a).
+       {:pattern PEq #a p1 p2} PEq #a p1 p2 <==> p1==p2)
