lib/FStar.Relational.fst
@@ -1,8 +1,3 @@
-(*--build-config
-    options:;
-    other-files:FStar.List.Tot.fst FStar.FunctionalExtensionality.fst FStar.Set.fst FStar.Heap.fst FStar.ST.fst FStar.All.fst FStar.List.fst
-  --*)
-
 module FStar.Relational
 open FStar.Heap
 
@@ -35,14 +30,14 @@ let op_Hat_Slash = rel_map2T (fun x y -> x / y)
 
 (* Some convenient list functions *)
 val tl_rel: #a:Type -> l:double (list a){is_Cons (R.l l) /\ is_Cons (R.r l)}-> Tot (double (list a))
-let tl_rel #a (R (_::xs) (_::ys)) = R xs ys
+let tl_rel (R (_::xs) (_::ys)) = R xs ys
 let cons_rel (R x y) (R xs ys) = R (x::xs) (y::ys) 
 (* Some convenient tuple functions *)
 let pair_rel (R a b) (R c d) = R (a,c) (b,d)
 let triple_rel (R a b) (R c d) (R e f) = R (a,c,e) (b,d,f)
-let fst_rel = rel_map1T fst 
-let snd_rel = rel_map1T snd 
- 
+let fst_rel = rel_map1T fst
+let snd_rel = rel_map1T snd
+
 (* Some convenient boolean functions *)
 let and_rel = rel_map2T (fun x y -> x && y)
 let or_rel = rel_map2T (fun x y -> x || y)
@@ -66,26 +61,26 @@ open FStar.Relational
 type heap2 = double heap
 
 new_effect STATE2 = STATE_h heap2
-let st2_Pre = st_pre_h heap2
-let st2_Post (a:Type) = st_post_h heap2 a
-let st2_WP (a:Type) = st_wp_h heap2 a
-effect ST2 (a:Type) (pre:st2_Pre) (post: (heap2 -> st2_Post a)) =
+kind ST2Pre = STPre_h heap2
+kind ST2Post (a:Type) = STPost_h heap2 a
+kind ST2WP (a:Type) = STWP_h heap2 a
+effect ST2 (a:Type) (pre:ST2Pre) (post: (heap2 -> ST2Post a)) =
     STATE2 a
-      (fun (p:st2_Post a) (h:heap2) -> pre h /\ (forall a h1. (pre h /\ post h a h1) ==> p a h1)) (* WP *)
-      (fun (p:st2_Post a) (h:heap2) -> (forall a h1. (pre h /\ post h a h1) ==> p a h1))          (* WLP *)
+      (fun (p:ST2Post a) (h:heap2) -> pre h /\ (forall a h1. (pre h /\ post h a h1) ==> p a h1)) (* WP *)
+      (fun (p:ST2Post a) (h:heap2) -> (forall a h1. (pre h /\ post h a h1) ==> p a h1))          (* WLP *)
 effect St2 (a:Type) = ST2 a (fun h -> True) (fun h0 r h1 -> True)
 sub_effect
-  DIV    ~> STATE2 = (fun (a:Type) (wp:pure_wp a) (p:st2_Post a) -> (fun h2 -> wp (fun a0 -> p a0 h2)))
+  DIV    ~> STATE2 = (fun (a:Type) (wp:PureWP a) (p:ST2Post a) -> (fun h2 -> wp (fun a0 -> p a0 h2)))
 
-(* construct a st2_WP from 2 st_wps *)
-type comp (a:Type) (b:Type) (wp0:st_wp a) (wp1:st_wp b) (p:((rel a b) -> heap2 -> Type)) (h2:heap2) =
+(* construct a ST2WP from 2 STWPs *)
+type comp (a:Type) (b:Type) (wp0:STWP a) (wp1:STWP b) (p:((rel a b) -> heap2 -> Type)) (h2:heap2) =
     wp0 (fun y0 h0 ->
       wp1 (fun y1 h1 -> p (R y0 y1) (R h0 h1))
       (R.r h2))
     (R.l h2)
 
-assume val compose2: #a0:Type -> #b0:Type -> #wp0:(a0 -> st_wp b0) -> #wlp0:(a0 -> st_wp b0)
-                  -> #a1:Type -> #b1:Type -> #wp1:(a1 -> st_wp b1) -> #wlp1:(a1 -> st_wp b1)
+assume val compose2: #a0:Type -> #b0:Type -> #wp0:(a0 -> STWP b0) -> #wlp0:(a0 -> STWP b0)
+                  -> #a1:Type -> #b1:Type -> #wp1:(a1 -> STWP b1) -> #wlp1:(a1 -> STWP b1)
                   -> =c0:(x0:a0 -> STATE b0 (wp0 x0) (wlp0 x0))
                   -> =c1:(x1:a1 -> STATE b1 (wp1 x1) (wlp1 x1))
                   -> x: rel a0 a1
@@ -93,13 +88,13 @@ assume val compose2: #a0:Type -> #b0:Type -> #wp0:(a0 -> st_wp b0) -> #wlp0:(a0 
                             (comp b0 b1 (wp0 (R.l x)) (wp1 (R.r x)))
                             (comp b0 b1 (wlp0 (R.l x)) (wlp1 (R.r x)))
 
-val compose2_self : #a:Type -> #b:Type -> #wp:(a -> st_wp b) -> #wlp:(a -> st_wp b)
+val compose2_self : #a:Type -> #b:Type -> #wp:(a -> STWP b) -> #wlp:(a -> STWP b)
                 -> =c:(x:a -> STATE b (wp x) (wlp x))
                 -> x: double a
                 -> STATE2 (double b)
                           (comp b b (wp (R.l x)) (wp (R.r x)))
                           (comp b b (wlp (R.l x)) (wlp (R.r x)))
-let compose2_self #a #b #wp #wlp f x = compose2 f f x
+let compose2_self f x = compose2 f f x
 
 (* Combine two ST2 statements A and B to create a new ST2 statement C where 
    the left side of C is equivalent to the left side of A and 
@@ -125,28 +120,28 @@ assume val cross : #a:Type -> #b:Type -> #c:Type -> #d:Type
 
 (* Create a ST statment from a ST2 statement by projection *)
 type decomp_l (a0:Type) (a1:Type) (b0:Type) (b1:Type) (al:a0)
-            (wp:(rel a0 a1 -> st2_WP (rel b0 b1))) (p:b0 -> heap -> Type) (hl:heap) = 
+            (wp:(rel a0 a1 -> ST2WP (rel b0 b1))) (p:b0 -> heap -> Type) (hl:heap) = 
     (exists (ar:a1) (hr:heap).
       wp (R al ar) (fun y2 h2 -> p (R.l y2) (R.l h2))
          (R hl hr))
 
 type decomp_r (a0:Type) (a1:Type) (b0:Type) (b1:Type) (ar:a1)
-            (wp:(rel a0 a1 -> st2_WP (rel b0 b1))) (p:b1 -> heap -> Type) (hr:heap) =
+            (wp:(rel a0 a1 -> ST2WP (rel b0 b1))) (p:b1 -> heap -> Type) (hr:heap) =
     (exists (al:a0) (hl:heap).
       wp (R al ar) (fun y2 h2 -> p (R.r y2) (R.r h2))
          (R hl hr))
 
 assume val project_l : #a0:Type -> #b0:Type -> #a1:Type -> #b1:Type
-                    -> #wp:(rel a0 a1 -> st2_WP (rel b0 b1))
-                    -> #wlp:(rel a0 a1 -> st2_WP (rel b0 b1))
+                    -> #wp:(rel a0 a1 -> ST2WP (rel b0 b1))
+                    -> #wlp:(rel a0 a1 -> ST2WP (rel b0 b1))
                     -> =c:(x:rel a0 a1 -> STATE2 (rel b0 b1) (wp x) (wlp x))
                     -> x:a0
                     -> STATE b0 (decomp_l a0 a1 b0 b1 x wp)
                                 (decomp_l a0 a1 b0 b1 x wlp)
 
 assume val project_r : #a0:Type -> #b0:Type -> #a1:Type -> #b1:Type
-                    -> #wp:(rel a0 a1 -> st2_WP (rel b0 b1))
-                    -> #wlp:(rel a0 a1 -> st2_WP (rel b0 b1))
+                    -> #wp:(rel a0 a1 -> ST2WP (rel b0 b1))
+                    -> #wlp:(rel a0 a1 -> ST2WP (rel b0 b1))
                     -> =c:(x:rel a0 a1 -> STATE2 (rel b0 b1) (wp x) (wlp x))
                     -> x:a1
                     -> STATE b1 (decomp_r a0 a1 b0 b1 x wp)
