lib/FStar.Seq.fst
@@ -1,7 +1,3 @@
-(*--build-config
-    options:--admit_fsi Set;
-    other-files: ext.fst FStar.Set.fsi seq.fsi
-  --*)
 (*
    Copyright 2008-2014 Nikhil Swamy and Microsoft Research
 
@@ -23,124 +19,142 @@
 module FStar.Seq
 #set-options "--initial_fuel 0 --max_fuel 0 --initial_ifuel 1 --max_ifuel 1"
 
-abstract type seq (a:Type) =
+(* Representation hidden from clients *)
+// type seq : Type -> Type
+type seq (a:Type) =
 | MkSeq: length:nat -> contents:(n:nat{n<length} -> Tot a) -> seq a
 
-(* Destructors *)
-abstract val length: #a:Type -> seq a -> Tot nat
-let length #a s = MkSeq.length s
+(* Operator for concatenation *)
+assume val op_At_Bar: #a:Type -> seq a -> seq a -> Tot (seq a)
 
-abstract val index:  #a:Type -> s:seq a -> i:nat{i < length s} -> Tot a
-let index #a s i = MkSeq.contents s i
+(* Primitive operations on sequences *)
+val length: #a:Type -> seq a -> Tot nat
+let length s = MkSeq.length s
+(*
+(match s with
+  | MkSeq l c -> l)
+*)
 
-abstract val create: #a:Type -> nat -> a -> Tot (seq a)
-let create #a len v =  MkSeq len (fun i -> v)
+val mkSeqContents : s:(seq 'a) -> n:nat{n<length s} -> Tot 'a
+let mkSeqContents s n = MkSeq.contents s n
+(*
+(match s with
+| MkSeq l c -> c n)
+*)
 
-private val exFalso0 : a:Type -> n:nat{n<0} -> Tot a
-let exFalso0 a n = ()
+val create: #a:Type -> nat -> a -> Tot (seq a)
+let create len v =  MkSeq len (fun i -> v)
 
-abstract val createEmpty: #a:Type -> Tot (s:(seq a){length s=0})
-let createEmpty #a = MkSeq 0 (fun i -> (exFalso0 a i))
+val exFalso0 : a:Type -> n:nat{n<0} -> Tot a
+let exFalso0 'a n = ()
 
-abstract val upd:    #a:Type -> s:seq a -> n:nat{n < length s} -> a ->  Tot (seq a)
-let upd #a s n v =
-  MkSeq (length s) (fun i -> if i=n then v else index s i)
+val createEmpty: #a:Type -> Tot (s:(seq a){length s=0})
+let createEmpty 'a =  (MkSeq 0 (fun i -> (exFalso0 'a i)))
 
-abstract val append: #a:Type -> seq a -> seq a -> Tot (seq a)
-let append #a s1 s2 =
+val index: #a:Type -> s:seq a -> i:nat{i < length s} -> Tot a
+let index s i = mkSeqContents s i
+
+val upd: #a:Type -> s:seq a -> n:nat{n < length s} -> a ->  Tot (seq a)
+let upd s n v =
+ MkSeq (length s) (fun i -> if i=n then v else (mkSeqContents s) i)
+
+val append: #a:Type -> seq a -> seq a -> Tot (seq a)
+let append s1 s2 =
   MkSeq (length s1 + length s2) (fun x -> if x < (length s1) then index s1 x else index s2 (x - (length s1)))
-let op_At_Bar (#a:Type) (s1:seq a) (s2:seq a) = append s1 s2
 
-abstract val slice:  #a:Type -> s:seq a -> i:nat -> j:nat{i <= j && j <= length s} -> Tot (seq a)
-let slice #a s i j = 
+val slice:  #a:Type -> s:seq a -> i:nat -> j:nat{i <= j && j <= length s} -> Tot (seq a)
+let slice s i j =
   MkSeq (j-i) (fun x -> index s (x + i))
 
 (* Lemmas about length *)
-abstract val lemma_create_len: #a:Type -> n:nat -> i:a -> Lemma
+val lemma_create_len: #a:Type -> n:nat -> i:a -> Lemma
   (requires True)
   (ensures (length (create n i) = n))
   [SMTPat (length (create n i))]
-let lemma_create_len #a n i   = ()
 
-abstract val lemma_len_upd: #a:Type -> n:nat -> v:a -> s:seq a{n < length s} -> Lemma
+val lemma_len_upd: #a:Type -> n:nat -> v:a -> s:seq a{n < length s} -> Lemma
   (requires True)
   (ensures (length (upd s n v) = length s))
   [SMTPat (length (upd s n v))]
-let lemma_len_upd #a n v s    = ()
 
-abstract val lemma_len_append: #a:Type -> s1:seq a -> s2:seq a -> Lemma
+val lemma_len_append: #a:Type -> s1:seq a -> s2:seq a -> Lemma
   (requires True)
   (ensures (length (append s1 s2) = length s1 + length s2))
   [SMTPat (length (append s1 s2))]
-let lemma_len_append #a s1 s2 = ()
 
-abstract val lemma_len_slice: #a:Type -> s:seq a -> i:nat -> j:nat{i <= j && j <= length s} -> Lemma
+val lemma_len_slice: #a:Type -> s:seq a -> i:nat -> j:nat{i <= j && j <= length s} -> Lemma
   (requires True)
   (ensures (length (slice s i j) = j - i))
   [SMTPat (length (slice s i j))]
-let lemma_len_slice #a s i j  = ()
+
+let lemma_create_len n i   = ()
+let lemma_len_upd n v s    = ()
+let lemma_len_append s1 s2 = ()
+let lemma_len_slice s i j  = ()
 
 (* Lemmas about index *)
-abstract val lemma_index_create: #a:Type -> n:nat -> v:a -> i:nat{i < n} -> Lemma
+val lemma_index_create: #a:Type -> n:nat -> v:a -> i:nat{i < n} -> Lemma
   (requires True)
   (ensures (index (create n v) i = v))
   [SMTPat (index (create n v) i)]
-let lemma_index_create #a n v i  = ()
 
-abstract val lemma_index_upd1: #a:Type -> s:seq a -> n:nat{n < length s} -> v:a -> Lemma
+val lemma_index_upd1: #a:Type -> s:seq a -> n:nat{n < length s} -> v:a -> Lemma
   (requires True)
   (ensures (index (upd s n v) n = v))
   [SMTPat (index (upd s n v) n)]
-let lemma_index_upd1 #a n v s    = ()
 
-abstract val lemma_index_upd2: #a:Type -> s:seq a -> n:nat{n < length s} -> v:a -> i:nat{i<>n /\ i < length s} -> Lemma
+val lemma_index_upd2: #a:Type -> s:seq a -> n:nat{n < length s} -> v:a -> i:nat{i<>n /\ i < length s} -> Lemma
   (requires True)
   (ensures (index (upd s n v) i = index s i))
   [SMTPat (index (upd s n v) i)]
-let lemma_index_upd2 #a n v s i  = ()
 
-abstract val lemma_index_app1: #a:Type -> s1:seq a -> s2:seq a -> i:nat{i < length s1} -> Lemma
+val lemma_index_app1: #a:Type -> s1:seq a -> s2:seq a -> i:nat{i < length s1} -> Lemma
   (requires True)
   (ensures (index (append s1 s2) i = index s1 i))
   [SMTPat (index (append s1 s2) i)]
-let lemma_index_app1 #a s1 s2 i  = ()
 
-abstract val lemma_index_app2: #a:Type -> s1:seq a -> s2:seq a -> i:nat{i < length s1 + length s2 /\ length s1 <= i} -> Lemma
+val lemma_index_app2: #a:Type -> s1:seq a -> s2:seq a -> i:nat{i < length s1 + length s2 /\ length s1 <= i} -> Lemma
   (requires True)
   (ensures (index (append s1 s2) i = index s2 (i - length s1)))
   [SMTPat (index (append s1 s2) i)]
-let lemma_index_app2 #a s2 s2 i  = ()
 
-abstract val lemma_index_slice: #a:Type -> s:seq a -> i:nat -> j:nat{i <= j /\ j <= length s} -> k:nat{k < j - i} -> Lemma
+val lemma_index_slice: #a:Type -> s:seq a -> i:nat -> j:nat{i <= j /\ j <= length s} -> k:nat{k < j - i} -> Lemma
   (requires True)
   (ensures (index (slice s i j) k = index s (k + i)))
   [SMTPat (index (slice s i j) k)]
-let lemma_index_slice #a s i j k = ()
 
-abstract type Eq (#a:Type) (s1:seq a) (s2:seq a) =
+let lemma_index_create n v i  = ()
+let lemma_index_upd1 n v s    = ()
+let lemma_index_upd2 n v s i  = ()
+let lemma_index_app1 s1 s2 i  = ()
+let lemma_index_app2 s2 s2 i  = ()
+let lemma_index_slice s i j k = ()
+
+//type Eq: #a:Type -> seq a -> seq a -> Type
+opaque type Eq (#a:Type) (s1:seq a) (s2:seq a) =
   (length s1 = length s2
    /\ (forall (i:nat{i < length s1}).{:pattern (index s1 i); (index s2 i)} (index s1 i == index s2 i)))
 
 (*This should be provable now*)
-(* private assume Extensionality: forall (a:Type) (s1:seq a) (s2:seq a).{:pattern (Eq s1 s2)} Eq s1 s2 <==> (s1=s2) *)
-abstract val lemma_eq_intro: #a:Type -> s1:seq a -> s2:seq a -> Lemma
+assume Extensionality: forall (a:Type) (s1:seq a) (s2:seq a).{:pattern (Eq s1 s2)} Eq s1 s2 <==> (s1=s2)
+
+(* Extensionality *)
+val lemma_eq_intro: #a:Type -> s1:seq a -> s2:seq a -> Lemma
      (requires (length s1 = length s2
                /\ (forall (i:nat{i < length s1}).{:pattern (index s1 i); (index s2 i)} (index s1 i == index s2 i))))
      (ensures (Eq s1 s2))
      [SMTPatT (Eq s1 s2)]
-let lemma_eq_intro #a s1 s2 = ()
 
-abstract val lemma_eq_refl: #a:Type -> s1:seq a -> s2:seq a -> Lemma
+val lemma_eq_refl: #a:Type -> s1:seq a -> s2:seq a -> Lemma
      (requires (s1 = s2))
      (ensures (Eq s1 s2))
      [SMTPatT (Eq s1 s2)]
-let lemma_eq_refl #a s1 s2  = ()
 
-abstract val lemma_eq_elim: #a:Type -> s1:seq a -> s2:seq a -> Lemma
+val lemma_eq_elim: #a:Type -> s1:seq a -> s2:seq a -> Lemma
      (requires (Eq s1 s2))
      (ensures (s1=s2))
      [SMTPatT (Eq s1 s2)]
-let lemma_eq_elim #a s1 s2  = ()
 
-
-
+let lemma_eq_intro s1 s2 = ()
+let lemma_eq_refl s1 s2  = ()
+let lemma_eq_elim s1 s2  = ()
