lib/FStar.SeqProperties.fst
@@ -1,8 +1,3 @@
-(*--build-config
-    options:--admit_fsi FStar.Set --admit_fsi FStar.Seq;
-    other-files:FStar.Classical.fst FStar.FunctionalExtensionality.fst FStar.Set.fsi seq.fsi
-  --*)
-
 (*
    Copyright 2008-2014 Nikhil Swamy and Microsoft Research
 
@@ -26,52 +21,52 @@ open FStar.Seq
 
 val lemma_append_inj_l: #a:Type -> s1:seq a -> s2:seq a -> t1:seq a -> t2:seq a{length s1 = length t1 /\ Eq (append s1 s2) (append t1 t2)} -> i:nat{i < length s1}
   -> Lemma (index s1 i == index t1 i)
-let lemma_append_inj_l #a s1 s2 t1 t2 i =
+let lemma_append_inj_l s1 s2 t1 t2 i =
   assert (index s1 i = (index (append s1 s2) i));
   assert (index t1 i = (index (append t1 t2) i))
 
 val lemma_append_inj_r: #a:Type -> s1:seq a -> s2:seq a -> t1:seq a -> t2:seq a{length s1 = length t1 /\ length s2 = length t2 /\ Eq (append s1 s2) (append t1 t2)} -> i:nat{i < length s2}
   -> Lemma (ensures  (index s2 i == index t2 i))
-let lemma_append_inj_r #a s1 s2 t1 t2 i =
+let lemma_append_inj_r s1 s2 t1 t2 i =
   assert (index s2 i = (index (append s1 s2) (i + length s1)));
   assert (index t2 i = (index (append t1 t2) (i + length t1)))
 
 val lemma_append_len_disj: #a:Type -> s1:seq a -> s2:seq a -> t1:seq a -> t2:seq a {(length s1 = length t1 \/ length s2 = length t2) /\ (Eq (append s1 s2) (append t1 t2))}
   -> Lemma (ensures (length s1 = length t1 /\ length s2 = length t2))
-let lemma_append_len_disj #a s1 s2 t1 t2 =
+let lemma_append_len_disj s1 s2 t1 t2 =
   cut (length (append s1 s2) == length s1 + length s2);
   cut (length (append t1 t2) == length t1 + length t2)
 
 val lemma_append_inj: #a:Type -> s1:seq a -> s2:seq a -> t1:seq a -> t2:seq a {length s1 = length t1 \/ length s2 = length t2}
   -> Lemma (requires (Eq (append s1 s2) (append t1 t2)))
            (ensures (Eq s1 t1 /\ Eq s2 t2))
-let lemma_append_inj #a s1 s2 t1 t2 =
+let lemma_append_inj s1 s2 t1 t2 =
   lemma_append_len_disj s1 s2 t1 t2;
-  Classical.forall_intro #a #(fun i -> index s1 i == index s1 i) (lemma_append_inj_l s1 s2 t1 t2);
+  Classical.forall_intro (lemma_append_inj_l s1 s2 t1 t2);
   Classical.forall_intro (lemma_append_inj_r s1 s2 t1 t2)
 
 val head: #a:Type -> s:seq a{length s > 0} -> Tot a
-let head #a s = index s 0
+let head s = index s 0
 
 val tail: #a:Type -> s:seq a{length s > 0} -> Tot (seq a)
-let tail #a s = slice s 1 (length s)
+let tail s = slice s 1 (length s)
 
 val cons: #a:Type -> a -> seq a -> Tot (seq a)
-let cons #a x s = append (create 1 x) s
+let cons x s = append (create 1 x) s
 
 val split: #a:Type -> s:seq a -> i:nat{(0 <= i /\ i <= length s)} -> Tot (seq a * seq a)
-let split #a s i = slice s 0 i, slice s i (length s)
+let split s i = slice s 0 i, slice s i (length s)
 
 val lemma_split : #a:Type -> s:seq a -> i:nat{(0 <= i /\ i <= length s)} -> Lemma
   (ensures (append (fst (split s i)) (snd (split s i)) = s))
-let lemma_split #a s i =
+let lemma_split s i =
   cut (Eq (append (fst (split s i)) (snd (split s i)))  s)
 
 val split_eq: #a:Type -> s:seq a -> i:nat{(0 <= i /\ i <= length s)} -> Pure
   (seq a * seq a)
   (requires True)
   (ensures (fun x -> (append (fst x) (snd x) = s)))
-let split_eq #a s i =
+let split_eq s i =
   let x = split s i in
   lemma_split s i;
   x
@@ -87,26 +82,26 @@ val mem: 'a -> seq 'a -> Tot bool
 let mem x l = count x l > 0
 
 val swap: #a:Type -> s:seq a -> i:nat{i<length s} -> j:nat{j<length s} -> Tot (seq a)
-let swap #a s i j = upd (upd s j (index s i)) i (index s j)
+let swap s i j = upd (upd s j (index s i)) i (index s j)
 
 val lemma_slice_append: #a:Type -> s1:seq a{length s1 >= 1} -> s2:seq a -> Lemma
   (ensures (Eq (append s1 s2) (append (slice s1 0 1) (append (slice s1 1 (length s1)) s2))))
-let lemma_slice_append #a s1 s2 = ()
+let lemma_slice_append s1 s2 = ()
 
 val lemma_append_cons: #a:Type -> s1:seq a{length s1 > 0} -> s2:seq a -> Lemma
   (requires True)
   (ensures (Eq (append s1 s2) (cons (head s1) (append (tail s1) s2))))
-let rec lemma_append_cons #a s1 s2 = ()
+let rec lemma_append_cons s1 s2 = ()
 
 val lemma_tl: #a:Type -> hd:a -> tl:seq a -> Lemma
   (ensures (Eq (tail (cons hd tl)) tl))
-let lemma_tl #a hd tl = ()
+let lemma_tl hd tl = ()
 
 val sorted: #a:Type
           -> (a -> a -> Tot bool)
           -> s:seq a
           -> Tot bool (decreases (length s))
-let rec sorted #a f s =
+let rec sorted f s =
   if length s <= 1
   then true
   else let hd = head s in
@@ -117,7 +112,7 @@ val lemma_append_count: #a:Type -> lo:seq a -> hi:seq a -> Lemma
   (requires True)
   (ensures (forall x. count x (append lo hi) = (count x lo + count x hi)))
   (decreases (length lo))
-let rec lemma_append_count #a lo hi =
+let rec lemma_append_count lo hi =
   if length lo = 0
   then cut (Eq (append lo hi) hi)
   else (cut (Eq (cons (head lo) (append (tail lo) hi))
@@ -130,17 +125,17 @@ let rec lemma_append_count #a lo hi =
 val lemma_append_count_aux: #a:Type -> x:a -> lo:seq a -> hi:seq a -> Lemma
   (requires True)
   (ensures (count x (append lo hi) = (count x lo + count x hi)))
-let lemma_append_count_aux #a x lo hi = lemma_append_count lo hi
+let lemma_append_count_aux x lo hi = lemma_append_count lo hi
 
 val lemma_mem_inversion: #a:Type -> s:seq a{length s > 0} -> Lemma
   (ensures (forall x. mem x s = (x=head s || mem x (tail s))))
-let lemma_mem_inversion #a s = ()
+let lemma_mem_inversion s = ()
 
 val lemma_mem_count: #a:Type -> s:seq a -> f:(a -> Tot bool) -> Lemma
   (requires (forall (i:nat{i<length s}). f (index s i)))
   (ensures (forall (x:a). mem x s ==> f x))
   (decreases (length s))
-let rec lemma_mem_count #a s f =
+let rec lemma_mem_count s f =
   if length s = 0
   then ()
   else (cut (forall (i:nat{i<length (tail s)}). index (tail s) i = index s (i + 1));
@@ -150,11 +145,11 @@ val lemma_count_slice: #a:Type -> s:seq a -> i:nat{i<=length s} -> Lemma
   (requires True)
   (ensures (forall x. count x s = count x (slice s 0 i) + count x (slice s i (length s))))
   (decreases (length s))
-let lemma_count_slice #a s i =
+let lemma_count_slice s i =
   cut (Eq s (append (slice s 0 i) (slice s i (length s))));
   lemma_append_count (slice s 0 i) (slice s i (length s))
 
-type total_order (a:Type) (f: (a -> a -> Tot bool)) =
+opaque logic type total_order (a:Type) (f: (a -> a -> Tot bool)) =
     (forall a. f a a)                                           (* reflexivity   *)
     /\ (forall a1 a2. (f a1 a2 /\ a1<>a2)  <==> not (f a2 a1))  (* anti-symmetry *)
     /\ (forall a1 a2 a3. f a1 a2 /\ f a2 a3 ==> f a1 a3)        (* transitivity  *)
@@ -169,7 +164,7 @@ val sorted_concat_lemma: #a:Type
                                                  /\ (mem y hi ==> f pivot y)))
                                (ensures (sorted f (append lo (cons pivot hi))))
                                (decreases (length lo))
-let rec sorted_concat_lemma #a f lo pivot hi =
+let rec sorted_concat_lemma f lo pivot hi =
   if length lo = 0
   then (cut (Eq (append lo (cons pivot hi)) (cons pivot hi));
         cut (Eq (tail (cons pivot hi)) hi))
@@ -178,7 +173,7 @@ let rec sorted_concat_lemma #a f lo pivot hi =
         lemma_tl (head lo) (append (tail lo) (cons pivot hi)))
 
 #set-options "--max_fuel 1 --initial_fuel 1 --z3timeout 20"
-val split_5 : #a:Type -> s:seq a -> i:nat -> j:nat{i < j && j < length s} -> Pure (seq (seq a))
+opaque val split_5 : #a:Type -> s:seq a -> i:nat -> j:nat{i < j && j < length s} -> Pure (seq (seq a))
   (requires True)
   (ensures (fun x ->
             ((length x = 5)
@@ -188,7 +183,7 @@ val split_5 : #a:Type -> s:seq a -> i:nat -> j:nat{i < j && j < length s} -> Pur
              /\ Eq (index x 2) (slice s (i+1) j)
              /\ Eq (index x 3) (slice s j (j + 1))
              /\ Eq (index x 4) (slice s (j + 1) (length s)))))
-let split_5 #a s i j = admit()
+let split_5 s i j = admit()
 (* this often fails with Unknown assertion failed *)
 (* let split_5 s i j = *)
 (*   let frag_lo, rest  = split_eq s i in *)
@@ -207,7 +202,7 @@ val lemma_swap_permutes_aux_frag_eq: #a:Type -> s:seq a -> i:nat{i<length s} -> 
                           -> Lemma (ensures (slice s i' j' = slice (swap s i j) i' j'
                                             /\ slice s i (i + 1) = slice (swap s i j) j (j + 1)
                                             /\ slice s j (j + 1) = slice (swap s i j) i (i + 1)))
-let lemma_swap_permutes_aux_frag_eq #a s i j i' j' =
+let lemma_swap_permutes_aux_frag_eq s i j i' j' =
   cut (Eq (slice s i' j') (slice (swap s i j) i' j'));
   cut (Eq (slice s i (i + 1))  (slice (swap s i j) j (j + 1)));
   cut (Eq (slice s j (j + 1))  (slice (swap s i j) i (i + 1)))
@@ -216,7 +211,7 @@ let lemma_swap_permutes_aux_frag_eq #a s i j i' j' =
 val lemma_swap_permutes_aux: #a:Type -> s:seq a -> i:nat{i<length s} -> j:nat{i <= j && j<length s} -> x:a -> Lemma
   (requires True)
   (ensures (count x s = count x (swap s i j)))
-let lemma_swap_permutes_aux #a s i j x =
+let lemma_swap_permutes_aux s i j x =
   if j=i
   then cut (Eq (swap s i j) s)
   else begin
@@ -244,133 +239,133 @@ let lemma_swap_permutes_aux #a s i j x =
   end
 
 #set-options "--max_fuel 0 --initial_fuel 0 --z3timeout 5"
-type permutation (a:Type) (s1:seq a) (s2:seq a) =
+opaque type permutation (a:Type) (s1:seq a) (s2:seq a) =
        (forall i. count i s1 = count i s2)
 val lemma_swap_permutes: #a:Type -> s:seq a -> i:nat{i<length s} -> j:nat{i <= j && j<length s} -> Lemma
   (permutation a s (swap s i j))
-let lemma_swap_permutes #a s i j = Classical.forall_intro (lemma_swap_permutes_aux s i j)
+let lemma_swap_permutes s i j = Classical.forall_intro (lemma_swap_permutes_aux s i j)
 
 
 #set-options "--max_fuel 1 --initial_fuel 1"
 val cons_perm: #a:Type -> tl:seq a -> s:seq a{length s > 0} ->
          Lemma (requires (permutation a tl (tail s)))
                (ensures (permutation a (cons (head s) tl) s))
-let cons_perm #a tl s = lemma_tl (head s) tl
+let cons_perm tl s = lemma_tl (head s) tl
 
 #set-options "--max_fuel 2 --initial_fuel 2"
 val lemma_mem_append : #a:Type -> s1:seq a -> s2:seq a
       -> Lemma (ensures (forall x. mem x (append s1 s2) <==> (mem x s1 || mem x s2)))
-let lemma_mem_append #a s1 s2 = lemma_append_count s1 s2
+let lemma_mem_append s1 s2 = lemma_append_count s1 s2
 
 val lemma_slice_cons: #a:Type -> s:seq a -> i:nat -> j:nat{i < j && j <= length s}
   -> Lemma (ensures (forall x. mem x (slice s i j) <==> (x = index s i || mem x (slice s (i + 1) j))))
-let lemma_slice_cons #a s i j =
+let lemma_slice_cons s i j =
   cut (Eq (slice s i j) (append (create 1 (index s i)) (slice s (i + 1) j)));
   lemma_mem_append (create 1 (index s i)) (slice s (i + 1) j)
 
 val lemma_slice_snoc: #a:Type -> s:seq a -> i:nat -> j:nat{i < j && j <= length s}
   -> Lemma (ensures (forall x. mem x (slice s i j) <==> (x = index s (j - 1) || mem x (slice s i (j - 1)))))
-let lemma_slice_snoc #a s i j =
+let lemma_slice_snoc s i j =
   cut (Eq (slice s i j) (append (slice s i (j - 1)) (create 1 (index s (j - 1)))));
   lemma_mem_append (slice s i (j - 1)) (create 1 (index s (j - 1)))
 
 val lemma_ordering_lo_snoc: #a:Type -> f:tot_ord a -> s:seq a -> i:nat -> j:nat{i <= j && j < length s} -> pv:a
    -> Lemma (requires ((forall y. mem y (slice s i j) ==> f y pv) /\ f (index s j) pv))
             (ensures ((forall y. mem y (slice s i (j + 1)) ==> f y pv)))
-let lemma_ordering_lo_snoc #a f s i j pv =
+let lemma_ordering_lo_snoc f s i j pv =
   cut (Eq (slice s i (j + 1)) (append (slice s i j) (create 1 (index s j))));
   lemma_mem_append (slice s i j) (create 1 (index s j))
 
 val lemma_ordering_hi_cons: #a:Type -> f:tot_ord a -> s:seq a -> back:nat -> len:nat{back < len && len <= length s} -> pv:a
    -> Lemma (requires ((forall y. mem y (slice s (back + 1) len) ==> f pv y) /\ f pv (index s back)))
             (ensures ((forall y. mem y (slice s back len) ==> f pv y)))
-let lemma_ordering_hi_cons #a f s back len pv =
+let lemma_ordering_hi_cons f s back len pv =
   cut (Eq (slice s back len) (append (create 1 (index s back)) (slice s (back + 1) len)));
   lemma_mem_append (create 1 (index s back)) (slice s (back + 1) len)
 
 #set-options "--max_fuel 0 --initial_fuel 0"
 val swap_frame_lo : #a:Type -> s:seq a -> lo:nat -> i:nat{lo <= i} -> j:nat{i <= j && j < length s}
      -> Lemma (ensures (slice s lo i == slice (swap s i j) lo i))
-let swap_frame_lo #a s lo i j = cut (Eq (slice s lo i) (slice (swap s i j) lo i))
+let swap_frame_lo s lo i j = cut (Eq (slice s lo i) (slice (swap s i j) lo i))
 
 val swap_frame_lo' : #a:Type -> s:seq a -> lo:nat -> i':nat {lo <= i'} -> i:nat{i' <= i} -> j:nat{i <= j && j < length s}
      -> Lemma (ensures (slice s lo i' == slice (swap s i j) lo i'))
-let swap_frame_lo' #a s lo i' i j = cut (Eq (slice s lo i') (slice (swap s i j) lo i'))
+let swap_frame_lo' s lo i' i j = cut (Eq (slice s lo i') (slice (swap s i j) lo i'))
 
 val swap_frame_hi : #a:Type -> s:seq a -> i:nat -> j:nat{i <= j} -> k:nat{j < k} -> hi:nat{k <= hi /\ hi <= length s}
      -> Lemma (ensures (slice s k hi == slice (swap s i j) k hi))
-let swap_frame_hi #a s i j k hi = cut (Eq (slice s k hi) (slice (swap s i j) k hi))
+let swap_frame_hi s i j k hi = cut (Eq (slice s k hi) (slice (swap s i j) k hi))
 
 val lemma_swap_slice_commute  : #a:Type -> s:seq a -> start:nat -> i:nat{start <= i} -> j:nat{i <= j} -> len:nat{j < len && len <= length s}
     -> Lemma (ensures (slice (swap s i j) start len == (swap (slice s start len) (i - start) (j - start))))
-let lemma_swap_slice_commute #a s start i j len = admit()
+let lemma_swap_slice_commute s start i j len = admit()
 (* this often fails with "assertion failed" *)
 (* let lemma_swap_slice_commute s start i j len = cut (Eq (slice (swap s i j) start len) (swap (slice s start len) (i - start) (j - start))) *)
 
 val lemma_swap_permutes_slice : #a:Type -> s:seq a -> start:nat -> i:nat{start <= i} -> j:nat{i <= j} -> len:nat{j < len && len <= length s}
    -> Lemma (ensures (permutation a (slice s start len) (slice (swap s i j) start len)))
-let lemma_swap_permutes_slice #a s start i j len =
+let lemma_swap_permutes_slice s start i j len =
   lemma_swap_slice_commute s start i j len;
   lemma_swap_permutes (slice s start len) (i - start) (j - start)
 
 #set-options "--initial_fuel 0 --max_fuel 0"
 (* replaces the [i,j) sub-sequence of s1 with the corresponding sub-sequence of s2 *)
 val splice: #a:Type -> s1:seq a -> i:nat -> s2:seq a{length s1=length s2} -> j:nat{i <= j /\ j <= (length s2)} -> Tot (seq a)
-let splice #a s1 i s2 j = Seq.append (slice s1 0 i) (Seq.append (slice s2 i j) (slice s1 j (length s1)))
+let splice s1 i s2 j = Seq.append (slice s1 0 i) (Seq.append (slice s2 i j) (slice s1 j (length s1)))
 
 val splice_refl : #a:Type -> s:seq a -> i:nat -> j:nat{i <= j && j <= length s}
   -> Lemma
   (ensures (s == splice s i s j))
-let splice_refl #a s i j = cut (Eq s (splice s i s j))
+let splice_refl s i j = cut (Eq s (splice s i s j))
 
 val lemma_swap_splice : #a:Type -> s:seq a -> start:nat -> i:nat{start <= i} -> j:nat{i <= j} -> len:nat{j < len && len <= length s}
    -> Lemma
         (ensures (swap s i j == splice s start (swap s i j) len))
-let lemma_swap_splice #a s start i j len = cut (Eq (swap s i j) (splice s start (swap s i j) len))
+let lemma_swap_splice s start i j len = cut (Eq (swap s i j) (splice s start (swap s i j) len))
 
 val lemma_seq_frame_hi: #a:Type -> s1:seq a -> s2:seq a{length s1 = length s2} -> i:nat -> j:nat{i <= j} -> m:nat{j <= m} -> n:nat{m < n && n <= length s1}
   -> Lemma
   (requires (s1 == (splice s2 i s1 j)))
   (ensures  ((slice s1 m n == slice s2 m n) /\ (index s1 m == index s2 m)))
-let lemma_seq_frame_hi #a s1 s2 i j m n =
+let lemma_seq_frame_hi s1 s2 i j m n =
   cut (Eq (slice s1 m n) (slice s2 m n))
 
 val lemma_seq_frame_lo: #a:Type -> s1:seq a -> s2:seq a{length s1 = length s2} -> i:nat -> j:nat{i <= j} -> m:nat{j < m} -> n:nat{m <= n && n <= length s1}
   -> Lemma
   (requires (s1 == (splice s2 m s1 n)))
   (ensures  ((slice s1 i j == slice s2 i j) /\ (index s1 j == index s2 j)))
-let lemma_seq_frame_lo #a s1 s2 i j m n =
+let lemma_seq_frame_lo s1 s2 i j m n =
   cut (Eq (slice s1 i j) (slice s2 i j))
 
 val lemma_tail_slice: #a:Type -> s:seq a -> i:nat -> j:nat{i < j && j <= length s}
   -> Lemma
   (ensures (tail (slice s i j) == slice s (i + 1) j))
-let lemma_tail_slice #a s i j =
+let lemma_tail_slice s i j =
   cut (Eq (tail (slice s i j)) (slice s (i + 1) j))
 
 val lemma_weaken_frame_right : #a:Type -> s1:seq a -> s2:seq a{length s1 = length s2} -> i:nat -> j:nat -> k:nat{i <= j && j <= k && k <= length s1}
   -> Lemma
   (requires (s1 == splice s2 i s1 j))
   (ensures (s1 == splice s2 i s1 k))
-let lemma_weaken_frame_right #a s1 s2 i j k = cut (Eq s1 (splice s2 i s1 k))
+let lemma_weaken_frame_right s1 s2 i j k = cut (Eq s1 (splice s2 i s1 k))
 
 val lemma_weaken_frame_left : #a:Type -> s1:seq a -> s2:seq a{length s1 = length s2} -> i:nat -> j:nat -> k:nat{i <= j && j <= k && k <= length s1}
   -> Lemma
   (requires (s1 == splice s2 j s1 k))
   (ensures (s1 == splice s2 i s1 k))
-let lemma_weaken_frame_left #a s1 s2 i j k = cut (Eq s1 (splice s2 i s1 k))
+let lemma_weaken_frame_left s1 s2 i j k = cut (Eq s1 (splice s2 i s1 k))
 
 val lemma_trans_frame : #a:Type -> s1:seq a -> s2:seq a -> s3:seq a{length s1 = length s2 /\ length s2 = length s3} -> i:nat -> j:nat{i <= j && j <= length s1}
   -> Lemma
   (requires ((s1 == splice s2 i s1 j) /\ s2 == splice s3 i s2 j))
   (ensures (s1 == splice s3 i s1 j))
-let lemma_trans_frame #a s1 s2 s3 i j = cut (Eq s1 (splice s3 i s1 j))
+let lemma_trans_frame s1 s2 s3 i j = cut (Eq s1 (splice s3 i s1 j))
 
 val lemma_weaken_perm_left: #a:Type -> s1:seq a -> s2:seq a{length s1 = length s2} -> i:nat -> j:nat -> k:nat{i <= j /\ j <= k /\ k <= length s1}
   -> Lemma
   (requires (s1 == splice s2 j s1 k /\ permutation a (slice s2 j k) (slice s1 j k)))
   (ensures (permutation a (slice s2 i k) (slice s1 i k)))
-let lemma_weaken_perm_left #a s1 s2 i j k =
+let lemma_weaken_perm_left s1 s2 i j k =
   cut (Eq (slice s2 i k) (append (slice s2 i j)
                                  (slice s2 j k)));
   cut (Eq (slice s1 i k) (append (slice s2 i j)
@@ -382,7 +377,7 @@ val lemma_weaken_perm_right: #a:Type -> s1:seq a -> s2:seq a{length s1 = length 
   -> Lemma
   (requires (s1 == splice s2 i s1 j /\ permutation a (slice s2 i j) (slice s1 i j)))
   (ensures (permutation a (slice s2 i k) (slice s1 i k)))
-let lemma_weaken_perm_right #a s1 s2 i j k =
+let lemma_weaken_perm_right s1 s2 i j k =
   cut (Eq (slice s2 i k) (append (slice s2 i j)
                                  (slice s2 j k)));
   cut (Eq (slice s1 i k) (append (slice s1 i j)
@@ -395,27 +390,28 @@ val lemma_trans_perm: #a:Type -> s1:seq a -> s2:seq a -> s3:seq a{length s1 = le
   (requires (permutation a (slice s1 i j) (slice s2 i j)
              /\ permutation a (slice s2 i j) (slice s3 i j)))
   (ensures (permutation a (slice s1 i j) (slice s3 i j)))
-let lemma_trans_perm #a s1 s2 s3 i j = ()
+let lemma_trans_perm s1 s2 s3 i j = ()
 
 
 (*New addtions, please review*)
 
 val snoc : #a:Type -> seq a -> a -> Tot (seq a)
-let snoc #a s x = Seq.append s (Seq.create 1 x)
+let snoc s x = Seq.append s (Seq.create 1 x)
 
-type found (i:nat) = True
+opaque logic type found (i:nat) = True
 
 val seq_find_aux : #a:Type -> f:(a -> Tot bool) -> l:seq a
                    -> ctr:nat{ctr <= Seq.length l}
                    -> Pure (option a)
                       (requires (forall (i:nat{ i < Seq.length l /\ i >= ctr}).
                                         not (f (Seq.index l i) )))
-                      (ensures (function 
-                                  | None -> forall (i:nat{i < Seq.length l}).  not (f (Seq.index l i))
-                                  | Some x -> f x /\  (exists (i:nat{i < Seq.length l}). //{:pattern (found i)}
-                                                            x = Seq.index l i)))
+                      (ensures (fun o -> (is_None o ==> (forall (i:nat{i < Seq.length l}).
+                                                         not (f (Seq.index l i))))
+                                      /\ (is_Some o ==> (f (Some.v o)
+                                                        /\ (exists (i:nat{i < Seq.length l}). //{:pattern (found i)}
+                                                            o = Some (Seq.index l i))))))
 
-let rec seq_find_aux #a f l ctr =
+let rec seq_find_aux f l ctr =
   match ctr with
   | 0 -> None
   | _ -> let i = ctr - 1 in
@@ -428,11 +424,12 @@ let rec seq_find_aux #a f l ctr =
 val seq_find: #a:Type -> f:(a -> Tot bool) -> l:seq a ->
                      Pure (option a)
                           (requires True)
-                          (ensures (function
-                                      | None -> forall (i:nat{i < Seq.length l}). not (f (Seq.index l i))
-                                      | Some x -> f x /\ (exists (i:nat{i < Seq.length l}).{:pattern (found i)}
-                                                          found i /\ x = Seq.index l i)))
+                          (ensures (fun o -> (is_None o ==> (forall (i:nat{i < Seq.length l}). not (f (Seq.index l i))))
+                                          /\ (is_Some o
+                                              ==> (f (Some.v o)
+                                                   /\ (exists (i:nat{i < Seq.length l}).{:pattern (found i)}
+                                                       found i /\ o = Some (Seq.index l i))))))
 
-let seq_find #a f l =
+let seq_find f l =
   admit ();
   seq_find_aux f l (Seq.length l)
