lib/prims.fst
@@ -1,5 +1,5 @@
 (*
-   Copyright 2008-2016 Nikhil Swamy and Microsoft Research
+   Copyright 2008-2014 Nikhil Swamy and Microsoft Research
 
    Licensed under the Apache License, Version 2.0 (the "License");
    you may not use this file except in compliance with the License.
@@ -14,112 +14,78 @@
    limitations under the License.
 *)
 module Prims
-(* False is the empty inductive type *)
-type False =
 
-(* True is the singleton inductive type *)
+kind Unop  = Type -> Type
+kind Binop = Type -> Type -> Type
+type bool
+logic type EqTyp : Type -> Type -> Type          (* infix binary '==' *)
+type Eq2 : #a:Type -> #b:Type -> a -> b -> Type    (* infix binary '==' *)
+opaque logic type b2t (b:bool) = (b == true)
+
+//We assume the Tot effect here; its definition appears a few lines below
+(* Primitive logical connectives *)
 type True =
   | T
-
-(* another singleton type, with its only inhabitant written '()'
-   we assume it is primitive, for convenient interop with other languages *)
-assume new type unit : Type0
-
-(*
-   infix binary '==';
-   proof irrelevant, heterogeneous equality in Type#0;
-   primitive (TODO: make it an inductive?)
-*)
-assume type Eq2 : #a:Type -> #b:Type -> a -> b -> Type0
-
-(* bool is a two element type with elements {'true', 'false'}
-   we assume it is primitive, for convenient interop with other languages *)
-assume new type bool : Type0
-
-(* bool-to-type coercion *)
-type b2t (b:bool) = (b == true)
-
-(* constructive conjunction *)
-type c_and  (p:Type) (q:Type) =
-  | And   : p -> q -> c_and p q
-
-(* '/\'  : specialized to Type#0 *)
-type l_and (p:Type0) (q:Type0) = c_and p q
-
-(* constructive disjunction *)
-type c_or   (p:Type) (q:Type) =
-  | Left  : p -> c_or p q
-  | Right : q -> c_or p q
-
-(* '\/'  : specialized to Type#0 *)
-type l_or (p:Type0) (q:Type0) = c_or p q
-
-(* '==>' : specialized to Type#0 *)
-type l_imp (p:Type0) (q:Type0) = p -> GTot q
-                                         (* ^^^ NB: The Tot effect is primitive;            *)
-				         (*         elaborated using PURE a few lines below *)
-(* infix binary '<==>' *)
-type l_iff (p:Type) (q:Type) = (p ==> q) /\ (q ==> p)
-
-(* prefix unary '~' *)
-type l_not (p:Type) = p ==> False
-
-type XOR (p:Type) (q:Type) = (p \/ q) /\ ~(p /\ q)
-
-type ITE (p:Type) (q:Type) (r:Type) = (p ==> q) /\ (~p ==> r)
-
-(* infix binary '<<'; a built-in well-founded partial order over all terms *)
-assume type precedes : #a:Type -> #b:Type -> a -> b -> Type0
-
-(* A coercion down to universe 0 *)
-type squash (p:Type) = u:unit{p}
-
-(* forall (x:a). p x : specialized to Type#0 *)
-type Forall (#a:Type) (p:a -> GTot Type0) = squash (x:a -> GTot (p x))
-
-(* dependent pairs DTuple2 in concrete syntax is '(x:a & b x)' *)
-type DTuple2 (a:Type)
-             (b:(a -> GTot Type)) =
-  | MkDTuple2: _1:a
-            -> _2:b _1
-            -> DTuple2 a b
-
-(* exists (x:a). p x : specialized to Type#0 *)
-type Exists (#a:Type) (p:a -> GTot Type0) = squash (x:a & p x)
+logic type False
+opaque type l_imp (p:Type) (q:Type) = p -> Tot q                (* infix binary '==>' *)
+type l_and  (p:Type) (q:Type) =
+  | And : p -> q -> (p /\ q)                                      (* infix binary '/\' *)
+type l_or   (p:Type) (q:Type) =                                 (* infix binary '\/' *)
+  | Left : p -> (p \/ q)
+  | Right : q -> (p \/ q)
+opaque type l_iff (p:Type) (q:Type) = (p ==> q) /\ (q ==> p)        (* infix binary '<==>' *)
+opaque type l_not (p:Type) = p ==> False                        (* prefix unary '~' *)
+opaque type Forall (#a:Type) (p:a -> Type) = x:a -> Tot (p x)   (* forall (x:a). p x *)
+type DTuple2: a:Type
+          ->  b:(a -> Type)
+          -> Type =
+  | MkDTuple2: #a:Type
+           ->  #b:(a -> Type)
+           -> _1:a
+           -> _2:b _1
+           -> DTuple2 a b
+opaque type Exists (#a:Type) (p:a -> Type) = x:a & p x          (* exists (x:a). p x *)
+logic type XOR (p:Type) (q:Type) = (p \/ q) /\ ~(p /\ q)
+opaque type ITE (p:Type) (q:Type) (r:Type) = (p ==> q) /\ (~p ==> r) (* if/then/else in concrete syntax *)
+logic type ForallTyp : (Type -> Type) -> Type (* Handled specially to support quantification over types of arbitrary kinds *)
+logic type ExistsTyp : (Type -> Type) -> Type (* Handled specially to support quantification over types of arbitrary kinds *)
+logic type Precedes : #a:Type -> #b:Type -> a -> b -> Type  (* a built-in well-founded partial order over all terms *)
 
 (* PURE effect *)
-let pure_pre = Type0
-let pure_post (a:Type) = a -> GTot Type0
-let pure_wp   (a:Type) = pure_post a -> GTot pure_pre
-
-inline let pure_return (a:Type) (x:a) (p:pure_post a) =
+kind PurePre = Type
+kind PurePost (a:Type) = a -> Type
+kind PureWP   (a:Type) = PurePost a -> PurePre
+type pure_return (a:Type) (x:a) (p:PurePost a) =
      p x
-inline let pure_bind_wlp (a:Type) (b:Type)
-                   (wlp1:pure_wp a) (wlp2:(a -> GTot (pure_wp b)))
-                   (p:pure_post b) =
+type pure_bind_wlp (a:Type) (b:Type)
+                   (wlp1:PureWP a) (wlp2:(a -> PureWP b))
+                   (p:PurePost b) =
      wlp1 (fun (x:a) -> wlp2 x p)
-inline let pure_bind_wp  (a:Type) (b:Type)
-                   (wp1:pure_wp a) (wlp1:pure_wp a)
-                   (wp2: (a -> GTot (pure_wp b))) (wlp2: (a -> GTot (pure_wp b))) =
+type pure_bind_wp  (a:Type) (b:Type)
+                   (wp1:PureWP a) (wlp1:PureWP a)
+                   (wp2: (a -> PureWP b)) (wlp2: (a -> PureWP b)) =
      pure_bind_wlp a b wp1 wp2
-inline let pure_if_then_else (a:Type) (p:Type) (wp_then:pure_wp a) (wp_else:pure_wp a) (post:pure_post a) =
-     ITE p (wp_then post) (wp_else post)
-inline let pure_ite_wlp (a:Type) (wlp_cases:pure_wp a) (post:pure_post a) =
+type pure_if_then_else (a:Type) (p:Type) (wp_then:PureWP a) (wp_else:PureWP a) (post:PurePost a) =
+     (if p
+      then wp_then post
+      else wp_else post)
+type pure_ite_wlp (a:Type) (wlp_cases:PureWP a) (post:PurePost a) =
      (forall (x:a). wlp_cases (fun (x':a) -> ~(Eq2 #a #a x x')) \/ post x)
-inline let pure_ite_wp (a:Type) (wlp_cases:pure_wp a) (wp_cases:pure_wp a) (post:pure_post a) =
+type pure_ite_wp (a:Type) (wlp_cases:PureWP a) (wp_cases:PureWP a) (post:PurePost a) =
      pure_ite_wlp a wlp_cases post
     /\ wp_cases (fun (x:a) -> True)
-inline let pure_wp_binop (a:Type) (wp1:pure_wp a) (op:(Type -> Type -> Type)) (wp2:pure_wp a) (p:pure_post a) =
+type pure_wp_binop (a:Type) (wp1:PureWP a) (op:(Type -> Type -> Type)) (wp2:PureWP a) (p:PurePost a) =
      op (wp1 p) (wp2 p)
-inline let pure_wp_as_type (a:Type) (wp:pure_wp a) = forall (p:pure_post a). wp p
-inline let pure_close_wp (a:Type) (b:Type) (wp:(b -> GTot (pure_wp a))) (p:pure_post a) = forall (b:b). wp b p
-inline let pure_assert_p (a:Type) (q:Type) (wp:pure_wp a) (p:pure_post a) = q /\ wp p
-inline let pure_assume_p (a:Type) (q:Type) (wp:pure_wp a) (p:pure_post a) = q ==> wp p
-inline let pure_null_wp  (a:Type) (p:pure_post a) = forall (x:a). p x
-inline let pure_trivial  (a:Type) (wp:pure_wp a) = wp (fun (x:a) -> True)
+type pure_wp_as_type (a:Type) (wp:PureWP a) = (forall (p:PurePost a). wp p)
+type pure_close_wp (a:Type) (b:Type) (wp:(b -> PureWP a)) (p:PurePost a) = (forall (b:b). wp b p)
+type pure_close_wp_t (a:Type) (wp:(Type -> PureWP a)) (p:PurePost a) = (forall (b:Type). wp b p)
+type pure_assert_p (a:Type) (q:Type) (wp:PureWP a) (p:PurePost a) = (q /\ wp p)
+type pure_assume_p (a:Type) (q:Type) (wp:PureWP a) (p:PurePost a) = (q ==> wp p)
+type pure_null_wp (a:Type) (p:PurePost a) = (forall (x:a). p x)
+type pure_trivial (a:Type) (wp:PureWP a) = wp (fun (x:a) -> True)
 
 total new_effect { (* The definition of the PURE effect is fixed; no user should ever change this *)
-  PURE : a:Type -> wp:pure_wp a -> wlp:pure_wp a -> Effect
+  PURE : a:Type -> wp:PureWP a -> wlp:PureWP a -> Effect
   with return       = pure_return
      ; bind_wlp     = pure_bind_wlp
      ; bind_wp      = pure_bind_wp
@@ -129,61 +95,63 @@ total new_effect { (* The definition of the PURE effect is fixed; no user should
      ; wp_binop     = pure_wp_binop
      ; wp_as_type   = pure_wp_as_type
      ; close_wp     = pure_close_wp
+     ; close_wp_t   = pure_close_wp_t
      ; assert_p     = pure_assert_p
      ; assume_p     = pure_assume_p
      ; null_wp      = pure_null_wp
      ; trivial      = pure_trivial
 }
-
-effect Pure (a:Type) (pre:pure_pre) (post:pure_post a) =
+effect Pure (a:Type) (pre:PurePre) (post:PurePost a) =
         PURE a
-             (fun (p:pure_post a) -> pre /\ (forall (x:a). post x ==> p x)) // pure_wp
-             (fun (p:pure_post a) -> forall (x:a). pre /\ post x ==> p x)   // WLP
-effect Admit (a:Type) = PURE a (fun (p:pure_post a) -> True) (fun (p:pure_post a) -> True)
-
-(* The primitive effect Tot is definitionally equal to an instance of PURE *)
+             (fun (p:PurePost a) -> pre /\ (forall (x:a). post x ==> p x)) (* PureWP *)
+             (fun (p:PurePost a) -> forall (x:a). pre /\ post x ==> p x)   (* WLP *)
+effect Admit (a:Type) = PURE a (fun (p:PurePost a) -> True) (fun (p:PurePost a) -> True)
 default effect Tot (a:Type) = PURE a (pure_null_wp a) (pure_null_wp a)
 
 total new_effect GHOST = PURE
-
-inline let purewp_id (a:Type) (wp:pure_wp a) = wp
-
 sub_effect
-  PURE ~> GHOST = purewp_id
-
-(* The primitive effect GTot is definitionally equal to an instance of GHOST *)
+  PURE ~> GHOST = fun (a:Type) (wp:PureWP a) -> wp
 default effect GTot (a:Type) = GHOST a (pure_null_wp a) (pure_null_wp a)
-
-effect Ghost (a:Type) (pre:Type) (post:pure_post a) =
+effect Ghost (a:Type) (pre:Type) (post:PurePost a) =
        GHOST a
-           (fun (p:pure_post a) -> pre /\ (forall (x:a). post x ==> p x))
-           (fun (p:pure_post a) -> forall (x:a). pre /\ post x ==> p x)
+           (fun (p:PurePost a) -> pre /\ (forall (x:a). post x ==> p x))
+           (fun (p:PurePost a) -> forall (x:a). pre /\ post x ==> p x)
 
-assume new type int : Type0
-assume val op_AmpAmp             : bool -> bool -> Tot bool
-assume val op_BarBar             : bool -> bool -> Tot bool
-assume val op_Negation           : bool -> Tot bool
-assume val op_Multiply           : int -> int -> Tot int
-assume val op_Subtraction        : int -> int -> Tot int
-assume val op_Addition           : int -> int -> Tot int
-assume val op_Minus              : int -> Tot int
-assume val op_LessThanOrEqual    : int -> int -> Tot bool
-assume val op_GreaterThan        : int -> int -> Tot bool
-assume val op_GreaterThanOrEqual : int -> int -> Tot bool
-assume val op_LessThan           : int -> int -> Tot bool
+type unit
+type int
+assume logic val op_AmpAmp             : bool -> bool -> Tot bool
+assume logic val op_BarBar             : bool -> bool -> Tot bool
+assume logic val op_Negation           : bool -> Tot bool
+assume logic val op_Multiply           : int -> int -> Tot int
+assume logic val op_Subtraction        : int -> int -> Tot int
+assume logic val op_Addition           : int -> int -> Tot int
+assume logic val op_Minus              : int -> Tot int
+assume logic val op_LessThanOrEqual    : int -> int -> Tot bool
+assume logic val op_GreaterThan        : int -> int -> Tot bool
+assume logic val op_GreaterThanOrEqual : int -> int -> Tot bool
+assume logic val op_LessThan           : int -> int -> Tot bool
 (* Primitive (structural) equality.
-   This still allows functions ... TODO: disallow functions *)
-assume val op_Equality :    'a -> 'a -> Tot bool
-assume val op_disEquality : 'a -> 'a -> Tot bool
-assume new type char   : Type0
-assume new type float  : Type0
-assume new type string : Type0
-assume new type exn : Type0
-type double = float
+   What about for function types? *)
+assume val op_Equality :    #a:Type -> a -> a -> Tot bool
+assume val op_disEquality : #a:Type -> a -> a -> Tot bool
 
+type int16 = i:int{i > -32769  /\ 32768 > i}
+type int32 = int
+type int64
+type uint8
+type uint16
+type uint32
+type uint64
+type char
+type float
+type string
+type array : Type -> Type
 assume val strcat : string -> string -> Tot string
-assume new type uint8 : Type0
+assume logic type LBL : string -> Type -> Type
+type exn
+type HashMultiMap : Type -> Type -> Type //needed for bootstrapping
 type byte = uint8
+type double = float
 
 type list (a:Type) =
   | Nil  : list a
@@ -192,9 +160,12 @@ type list (a:Type) =
 type pattern =
   | SMTPat   : #a:Type -> a -> pattern
   | SMTPatT  : a:Type -> pattern
-//  | SMTPatOr : list (list pattern) -> pattern //TODO: rechecking this fails some universe checks
+  | SMTPatOr : list (list pattern) -> pattern
 
-assume type decreases : #a:Type -> a -> Type0
+assume type decreases : #a:Type -> a -> Type
+
+effect Lemma (a:Type) (pre:Type) (post:Type) (pats:list pattern) =
+       Pure a pre (fun r -> post)
 
 (*
    Lemma is desugared specially. You can write:
@@ -202,10 +173,6 @@ assume type decreases : #a:Type -> a -> Type0
      Lemma phi                 for   Lemma (requires True) phi []
      Lemma t1..tn              for   Lemma unit t1..tn
 *)
-effect Lemma (a:Type) (pre:Type) (post:Type) (pats:list pattern) =
-       Pure a pre (fun r -> post)
-
-
 type option (a:Type) =
   | None : option a
   | Some : v:a -> option a
@@ -220,80 +187,81 @@ type result (a:Type) =
   | Err : msg:string -> result a
 
 new_effect DIV = PURE
-sub_effect PURE ~> DIV  = purewp_id
-
-effect Div (a:Type) (pre:pure_pre) (post:pure_post a) =
+effect Div (a:Type) (pre:PurePre) (post:PurePost a) =
        DIV a
-           (fun (p:pure_post a) -> pre /\ (forall a. post a ==> p a)) (* WP *)
-           (fun (p:pure_post a) -> forall a. pre /\ post a ==> p a)   (* WLP *)
+           (fun (p:PurePost a) -> pre /\ (forall a. post a ==> p a)) (* WP *)
+           (fun (p:PurePost a) -> forall a. pre /\ post a ==> p a)   (* WLP *)
 
 default effect Dv (a:Type) =
-     DIV a (fun (p:pure_post a) -> (forall (x:a). p x))
-           (fun (p:pure_post a) -> (forall (x:a). p x))
+     DIV a (fun (p:PurePost a) -> (forall (x:a). p x))
+           (fun (p:PurePost a) -> (forall (x:a). p x))
 
+kind STPre_h  (heap:Type)          = heap -> Type
+kind STPost_h (heap:Type) (a:Type) = a -> heap-> Type
+kind STWP_h   (heap:Type) (a:Type) = STPost_h heap a -> STPre_h heap
 
-let st_pre_h  (heap:Type)          = heap -> GTot Type0
-let st_post_h (heap:Type) (a:Type) = a -> heap -> GTot Type0
-let st_wp_h   (heap:Type) (a:Type) = st_post_h heap a -> Tot (st_pre_h heap)
-
-inline let st_return        (heap:Type) (a:Type)
-                            (x:a) (p:st_post_h heap a) =
+type st_return        (heap:Type) (a:Type)
+                      (x:a) (p:STPost_h heap a) =
      p x
-inline let st_bind_wp       (heap:Type) (a:Type) (b:Type)
-                            (wp1:st_wp_h heap a) (wlp1:st_wp_h heap a)
-                            (wp2:(a -> GTot (st_wp_h heap b))) (wlp2:(a -> GTot (st_wp_h heap b)))
-                            (p:st_post_h heap b) (h0:heap) =
-     wp1 (fun a h1 -> wp2 a p h1) h0
-inline let st_bind_wlp      (heap:Type) (a:Type) (b:Type)
-                             (wlp1:st_wp_h heap a) (wlp2:(a -> GTot (st_wp_h heap b)))
-                             (p:st_post_h heap b) (h0:heap) =
-     wlp1 (fun a h1 -> wlp2 a p h1) h0
-inline let st_if_then_else  (heap:Type) (a:Type) (p:Type)
-                             (wp_then:st_wp_h heap a) (wp_else:st_wp_h heap a)
-                             (post:st_post_h heap a) (h0:heap) =
-     ITE p
-        (wp_then post h0)
-	(wp_else post h0)
-inline let st_ite_wlp       (heap:Type) (a:Type)
-                             (wlp_cases:st_wp_h heap a)
-                             (post:st_post_h heap a) (h0:heap) =
+type st_bind_wp       (heap:Type) (a:Type) (b:Type)
+                      (wp1:STWP_h heap a) (wlp1:STWP_h heap a)
+                      (wp2:(a -> STWP_h heap b)) (wlp2:(a -> STWP_h heap b))
+                      (p:STPost_h heap b) (h0:heap) =
+     wp1 (fun a -> wp2 a p) h0
+type st_bind_wlp      (heap:Type) (a:Type) (b:Type)
+                      (wlp1:STWP_h heap a) (wlp2:(a -> STWP_h heap b))
+                      (p:STPost_h heap b) (h0:heap) =
+     wlp1 (fun a -> wlp2 a p) h0
+type st_if_then_else  (heap:Type) (a:Type) (p:Type)
+                      (wp_then:STWP_h heap a) (wp_else:STWP_h heap a)
+                      (post:STPost_h heap a) (h0:heap) =
+     (if p
+      then wp_then post h0
+      else wp_else post h0)
+type st_ite_wlp       (heap:Type) (a:Type)
+                      (wlp_cases:STWP_h heap a)
+                      (post:STPost_h heap a) (h0:heap) =
      (forall (a:a) (h:heap).
            wlp_cases (fun a1 h1 -> a=!=a1 \/ h=!=h1) h0
         \/ post a h)
-inline let st_ite_wp        (heap:Type) (a:Type)
-                             (wlp_cases:st_wp_h heap a) (wp_cases:st_wp_h heap a)
-                             (post:st_post_h heap a) (h0:heap) =
+type st_ite_wp        (heap:Type) (a:Type)
+                      (wlp_cases:STWP_h heap a) (wp_cases:STWP_h heap a)
+                      (post:STPost_h heap a) (h0:heap) =
      st_ite_wlp heap a wlp_cases post h0
      /\ wp_cases (fun a h_ -> True) h0
-inline let st_wp_binop      (heap:Type) (a:Type)
-                             (wp1:st_wp_h heap a)
-                             (op:(Type -> Type -> GTot Type))
-                             (wp2:st_wp_h heap a)
-                             (p:st_post_h heap a) (h:heap) =
+type st_wp_binop      (heap:Type) (a:Type)
+                      (wp1:STWP_h heap a)
+                      (op:(Type -> Type -> Type))
+                      (wp2:STWP_h heap a)
+                      (p:STPost_h heap a) (h:heap) =
      op (wp1 p h) (wp2 p h)
-inline let st_wp_as_type    (heap:Type) (a:Type) (wp:st_wp_h heap a) =
-     (forall (p:st_post_h heap a) (h:heap). wp p h)
-inline let st_close_wp      (heap:Type) (a:Type) (b:Type)
-                             (wp:(b -> GTot (st_wp_h heap a)))
-                             (p:st_post_h heap a) (h:heap) =
+type st_wp_as_type    (heap:Type) (a:Type) (wp:STWP_h heap a) =
+     (forall (p:STPost_h heap a) (h:heap). wp p h)
+type st_close_wp      (heap:Type) (a:Type) (b:Type)
+                      (wp:(b -> STWP_h heap a))
+                      (p:STPost_h heap a) (h:heap) =
      (forall (b:b). wp b p h)
-inline let st_assert_p      (heap:Type) (a:Type) (p:Type)
-                             (wp:st_wp_h heap a)
-                             (q:st_post_h heap a) (h:heap) =
+type st_close_wp_t    (heap:Type) (a:Type)
+                      (wp:(Type -> STWP_h heap a))
+                      (p:STPost_h heap a) (h:heap) =
+     (forall (b:Type). wp b p h)
+type st_assert_p      (heap:Type) (a:Type) (p:Type)
+                      (wp:STWP_h heap a)
+                      (q:STPost_h heap a) (h:heap) =
      p /\ wp q h
-inline let st_assume_p      (heap:Type) (a:Type) (p:Type)
-                             (wp:st_wp_h heap a)
-                             (q:st_post_h heap a) (h:heap) =
+type st_assume_p      (heap:Type) (a:Type) (p:Type)
+                      (wp:STWP_h heap a)
+                      (q:STPost_h heap a) (h:heap) =
      p ==> wp q h
-inline let st_null_wp       (heap:Type) (a:Type)
-                             (p:st_post_h heap a) (h:heap) =
+type st_null_wp       (heap:Type) (a:Type)
+                      (p:STPost_h heap a) (h:heap) =
      (forall (x:a) (h:heap). p x h)
-inline let st_trivial       (heap:Type) (a:Type)
-                             (wp:st_wp_h heap a) =
+type st_trivial       (heap:Type) (a:Type)
+                      (wp:STWP_h heap a) =
      (forall h0. wp (fun r h1 -> True) h0)
 
 new_effect {
-  STATE_h (heap:Type) : result:Type -> wp:st_wp_h heap result -> wlp:st_wp_h heap result -> Effect
+  STATE_h (heap:Type) : result:Type -> wp:STWP_h heap result -> wlp:STWP_h heap result -> Effect
   with return       = st_return heap
      ; bind_wp      = st_bind_wp heap
      ; bind_wlp     = st_bind_wlp heap
@@ -303,6 +271,7 @@ new_effect {
      ; wp_binop     = st_wp_binop heap
      ; wp_as_type   = st_wp_as_type heap
      ; close_wp     = st_close_wp heap
+     ; close_wp_t   = st_close_wp_t heap
      ; assert_p     = st_assert_p heap
      ; assume_p     = st_assume_p heap
      ; null_wp      = st_null_wp heap
@@ -310,41 +279,40 @@ new_effect {
 }
 
 (* Effect EXCEPTION *)
-let ex_pre  = Type0
-let ex_post (a:Type) = result a -> GTot Type0
-let ex_wp   (a:Type) = ex_post a -> GTot ex_pre
-inline let ex_return   (a:Type) (x:a) (p:ex_post a) = p (V x)
-inline let ex_bind_wlp (a:Type) (b:Type) (wlp1:ex_wp a) (wlp2:(a -> GTot (ex_wp b))) (p:ex_post b) =
-   (forall (rb:result b). p rb \/ wlp1 (fun ra1 -> if is_V ra1
-                                          then wlp2 (V.v ra1) (fun rb2 -> rb2=!=rb)
-                                          else ra1 =!= rb))
-inline let ex_bind_wp (a:Type) (b:Type)
-		       (wp1:ex_wp a) (wlp1:ex_wp a)
-		       (wp2:(a -> GTot (ex_wp b))) (wlp2:(a -> GTot (ex_wp b))) (p:ex_post b) =
+kind ExPre  = Type
+kind ExPost (a:Type) = result a -> Type
+kind ExWP   (a:Type) = ExPost a -> ExPre
+type ex_return (a:Type) (x:a) (p:ExPost a) = p (V x)
+type ex_bind_wlp (a:Type) (b:Type) (wlp1:ExWP a) (wlp2:(a -> ExWP b)) (p:ExPost b) =
+   (forall (rb:result b). p rb \/ wlp1 (fun ra1 -> if b2t (is_V ra1)
+                                                      then wlp2 (V.v ra1) (fun rb2 -> rb2=!=rb)
+                                                      else  ra1 =!= rb))
+type ex_bind_wp (a:Type) (b:Type) (wp1:ExWP a) (wlp1:ExWP a) (wp2:(a -> ExWP b)) (wlp2:(a -> ExWP b)) (p:ExPost b) =
    ex_bind_wlp a b wlp1 wlp2 p
-   /\ wp1 (fun ra1 -> if is_V ra1
-                   then wp2 (V.v ra1) (fun rb2 -> True)
-                   else True)
-inline let ex_if_then_else (a:Type) (p:Type) (wp_then:ex_wp a) (wp_else:ex_wp a) (post:ex_post a) =
-   ITE p
-       (wp_then post)
-       (wp_else post)
-inline let ex_ite_wlp  (a:Type) (wlp_cases:ex_wp a) (post:ex_post a) =
+   /\ wp1 (fun ra1 -> (ITE (b2t (is_V ra1))
+                            (wp2 (V.v ra1) (fun rb2 -> True))
+                             True))
+type ex_if_then_else (a:Type) (p:Type) (wp_then:ExWP a) (wp_else:ExWP a) (post:ExPost a) =
+   (if p
+    then wp_then post
+    else wp_else post)
+type ex_ite_wlp  (a:Type) (wlp_cases:ExWP a) (post:ExPost a) =
     (forall (a:result a). wlp_cases (fun a1 -> a=!=a1) \/ post a)
-inline let ex_ite_wp (a:Type) (wlp_cases:ex_wp a) (wp_cases:ex_wp a) (post:ex_post a) =
+type ex_ite_wp (a:Type) (wlp_cases:ExWP a) (wp_cases:ExWP a) (post:ExPost a) =
     ex_ite_wlp a wlp_cases post
     /\ wp_cases (fun ra2 -> True)
-inline let ex_wp_binop (a:Type) (wp1:ex_wp a) (op:(Type -> Type -> GTot Type)) (wp2:ex_wp a) (p:ex_post a) =
+type ex_wp_binop (a:Type) (wp1:ExWP a) (op:(Type -> Type -> Type)) (wp2:ExWP a) (p:ExPost a) =
    op (wp1 p) (wp2 p)
-inline let ex_wp_as_type (a:Type) (wp:ex_wp a) = (forall (p:ex_post a). wp p)
-inline let ex_close_wp (a:Type) (b:Type) (wp:(b -> GTot (ex_wp a))) (p:ex_post a) = (forall (b:b). wp b p)
-inline let ex_assert_p (a:Type) (q:Type) (wp:ex_wp a) (p:ex_post a) = (q /\ wp p)
-inline let ex_assume_p (a:Type) (q:Type) (wp:ex_wp a) (p:ex_post a) = (q ==> wp p)
-inline let ex_null_wp (a:Type) (p:ex_post a) = (forall (r:result a). p r)
-inline let ex_trivial (a:Type) (wp:ex_wp a) = wp (fun r -> True)
+type ex_wp_as_type (a:Type) (wp:ExWP a) = (forall (p:ExPost a). wp p)
+type ex_close_wp (a:Type) (b:Type) (wp:(b -> ExWP a)) (p:ExPost a) = (forall (b:b). wp b p)
+type ex_close_wp_t (a:Type) (wp:(Type -> ExWP a)) (p:ExPost a)  = (forall (b:Type). wp b p)
+type ex_assert_p (a:Type) (q:Type) (wp:ExWP a) (p:ExPost a) = (q /\ wp p)
+type ex_assume_p (a:Type) (q:Type) (wp:ExWP a) (p:ExPost a) = (q ==> wp p)
+type ex_null_wp (a:Type) (p:ExPost a) = (forall (r:result a). p r)
+type ex_trivial (a:Type) (wp:ExWP a) = wp (fun r -> True)
 
 new_effect {
-  EXN : result:Type -> wp:ex_wp result -> wlp:ex_wp result -> Effect
+  EXN : result:Type -> wp:ExWP result -> wlp:ExWP result -> Effect
   with
     return       = ex_return
   ; bind_wlp     = ex_bind_wlp
@@ -355,75 +323,78 @@ new_effect {
   ; wp_binop     = ex_wp_binop
   ; wp_as_type   = ex_wp_as_type
   ; close_wp     = ex_close_wp
+  ; close_wp_t   = ex_close_wp_t
   ; assert_p     = ex_assert_p
   ; assume_p     = ex_assume_p
   ; null_wp      = ex_null_wp
   ; trivial      = ex_trivial
 }
-effect Exn (a:Type) (pre:ex_pre) (post:ex_post a) =
+effect Exn (a:Type) (pre:ExPre) (post:ExPost a) =
        EXN a
-         (fun (p:ex_post a) -> pre /\ (forall (r:result a). (pre /\ post r) ==> p r)) (* WP *)
-         (fun (p:ex_post a) -> (forall (r:result a). (pre /\ post r) ==> p r))       (* WLP *)
-inline let lift_div_exn (a:Type) (wp:pure_wp a) (p:ex_post a) = wp (fun a -> p (V a))
-sub_effect DIV ~> EXN = lift_div_exn
+         (fun (p:ExPost a) -> pre /\ (forall (r:result a). (pre /\ post r) ==> p r)) (* ExWP *)
+         (fun (p:ExPost a) -> (forall (r:result a). (pre /\ post r) ==> p r))         (* WLP *)
 default effect Ex (a:Type) = Exn a True (fun v -> True)
 
-let all_pre_h  (h:Type)           = h -> GTot Type
-let all_post_h (h:Type) (a:Type)  = result a -> h -> GTot Type
-let all_wp_h   (h:Type) (a:Type)  = all_post_h h a -> Tot (all_pre_h h)
+kind AllPre_h  (h:Type)           = h -> Type
+kind AllPost_h (h:Type) (a:Type)  = result a -> h -> Type
+kind AllWP_h   (h:Type) (a:Type)  = AllPost_h h a -> AllPre_h h
 
-inline let all_return  (heap:Type) (a:Type) (x:a) (p:all_post_h heap a) = p (V x)
-inline let all_bind_wp (heap:Type) (a:Type) (b:Type)
-                        (wp1:all_wp_h heap a) (wlp1:all_wp_h heap a)
-                        (wp2:(a -> GTot (all_wp_h heap b))) (wlp2:(a -> GTot (all_wp_h heap b)))
-                        (p:all_post_h heap b) (h0:heap) =
-   (wp1 (fun ra h1 -> is_V ra ==> wp2 (V.v ra) p h1) h0)
-inline let all_bind_wlp (heap:Type) (a:Type) (b:Type)
-                         (wlp1:all_wp_h heap a) (wlp2:(a -> GTot (all_wp_h heap b)))
-                         (p:all_post_h heap b) (h0:heap) =
+type all_return  (heap:Type) (a:Type) (x:a) (p:AllPost_h heap a) = p (V x)
+type all_bind_wp (heap:Type) (a:Type) (b:Type)
+                 (wp1:AllWP_h heap a) (wlp1:AllWP_h heap a)
+                 (wp2:(a -> AllWP_h heap b)) (wlp2:(a -> AllWP_h heap b))
+                 (p:AllPost_h heap b) (h0:heap) =
+   (wp1 (fun ra h1 -> b2t(is_V ra) ==> wp2 (V.v ra) p h1) h0)
+type all_bind_wlp (heap:Type) (a:Type) (b:Type)
+                  (wlp1:AllWP_h heap a) (wlp2:(a -> AllWP_h heap b))
+                  (p:AllPost_h heap b) (h0:heap) =
    (forall rb h. wlp1 (fun ra h1 ->
-       if is_V ra
+       if b2t (is_V ra)
        then wlp2 (V.v ra) (fun rb2 h2 -> rb=!=rb2 \/ h=!=h2) h1
        else rb=!=ra \/ h=!=h1) h0 \/ p rb h)
-inline let all_if_then_else (heap:Type) (a:Type) (p:Type)
-                             (wp_then:all_wp_h heap a) (wp_else:all_wp_h heap a)
-                             (post:all_post_h heap a) (h0:heap) =
-   ITE p
-       (wp_then post h0)
-       (wp_else post h0)
-inline let all_ite_wlp  (heap:Type) (a:Type)
-                         (wlp_cases:all_wp_h heap a)
-                         (post:all_post_h heap a) (h0:heap) =
+type all_if_then_else (heap:Type) (a:Type) (p:Type)
+                      (wp_then:AllWP_h heap a) (wp_else:AllWP_h heap a)
+                      (post:AllPost_h heap a) (h0:heap) =
+   (if p
+    then wp_then post h0
+    else wp_else post h0)
+type all_ite_wlp  (heap:Type) (a:Type)
+                  (wlp_cases:AllWP_h heap a)
+                  (post:AllPost_h heap a) (h0:heap) =
      (forall (ra:result a) (h:heap). wlp_cases (fun ra2 h2 -> ra=!=ra2 \/ h=!=h2) h0 \/ post ra h)
-inline let all_ite_wp (heap:Type) (a:Type)
-                       (wlp_cases:all_wp_h heap a) (wp_cases:all_wp_h heap a)
-                       (post:all_post_h heap a) (h0:heap) =
+type all_ite_wp (heap:Type) (a:Type)
+                (wlp_cases:AllWP_h heap a) (wp_cases:AllWP_h heap a)
+                (post:AllPost_h heap a) (h0:heap) =
      (forall (ra:result a) (h:heap). wlp_cases (fun ra2 h2 -> ra=!=ra2 \/ h=!=h2) h0 \/ post ra h)
       /\ wp_cases (fun _a _b -> True) h0
-inline let all_wp_binop (heap:Type) (a:Type)
-                         (wp1:all_wp_h heap a) (op:(Type -> Type -> GTot Type))
-                         (wp2:all_wp_h heap a) (p:all_post_h heap a) (h:heap) =
+type all_wp_binop (heap:Type) (a:Type)
+                  (wp1:AllWP_h heap a) (op:(Type -> Type -> Type))
+                  (wp2:AllWP_h heap a) (p:AllPost_h heap a) (h:heap) =
      op (wp1 p h) (wp2 p h)
-inline let all_wp_as_type (heap:Type) (a:Type) (wp:all_wp_h heap a) =
-    (forall (p:all_post_h heap a) (h:heap). wp p h)
-inline let all_close_wp (heap:Type) (a:Type) (b:Type)
-                         (wp:(b -> GTot (all_wp_h heap a)))
-                         (p:all_post_h heap a) (h:heap) =
+type all_wp_as_type (heap:Type) (a:Type) (wp:AllWP_h heap a) =
+    (forall (p:AllPost_h heap a) (h:heap). wp p h)
+type all_close_wp (heap:Type) (a:Type) (b:Type)
+                  (wp:(b -> AllWP_h heap a))
+                  (p:AllPost_h heap a) (h:heap) =
     (forall (b:b). wp b p h)
-inline let all_assert_p (heap:Type) (a:Type) (p:Type)
-                         (wp:all_wp_h heap a) (q:all_post_h heap a) (h:heap) =
+type all_close_wp_t (heap:Type) (a:Type)
+                    (wp:(Type -> AllWP_h heap a))
+                    (p:AllPost_h heap a) (h:heap) =
+    (forall (b:Type). wp b p h)
+type all_assert_p (heap:Type) (a:Type) (p:Type)
+                  (wp:AllWP_h heap a) (q:AllPost_h heap a) (h:heap) =
     p /\ wp q h
-inline let all_assume_p (heap:Type) (a:Type) (p:Type)
-                         (wp:all_wp_h heap a) (q:all_post_h heap a) (h:heap) =
+type all_assume_p (heap:Type) (a:Type) (p:Type)
+                  (wp:AllWP_h heap a) (q:AllPost_h heap a) (h:heap) =
     p ==> wp q h
-inline let all_null_wp (heap:Type) (a:Type)
-                        (p:all_post_h heap a) (h0:heap) =
+type all_null_wp (heap:Type) (a:Type)
+                 (p:AllPost_h heap a) (h0:heap) =
     (forall (a:result a) (h:heap). p a h)
-inline let all_trivial (heap:Type) (a:Type) (wp:all_wp_h heap a) =
+type all_trivial (heap:Type) (a:Type) (wp:AllWP_h heap a) =
     (forall (h0:heap). wp (fun r h1 -> True) h0)
 
 new_effect {
-  ALL_h (heap:Type) : a:Type -> wp:all_wp_h heap a -> wlp:all_wp_h heap a -> Effect
+  ALL_h (heap:Type) : a:Type -> wp:AllWP_h heap a -> wlp:AllWP_h heap a -> Effect
   with
     return       = all_return       heap
   ; bind_wp      = all_bind_wp      heap
@@ -434,34 +405,34 @@ new_effect {
   ; wp_binop     = all_wp_binop     heap
   ; wp_as_type   = all_wp_as_type   heap
   ; close_wp     = all_close_wp     heap
+  ; close_wp_t   = all_close_wp_t   heap
   ; assert_p     = all_assert_p     heap
   ; assume_p     = all_assume_p     heap
   ; null_wp      = all_null_wp      heap
   ; trivial      = all_trivial      heap
+
 }
 
-
-
-
+sub_effect
+  PURE  ~> DIV   = fun (a:Type) (wp:PureWP a) (p:PurePost a) -> wp (fun a -> p a)
+sub_effect
+  DIV   ~> EXN   = fun (a:Type) (wp:PureWP a) (p:ExPost a) -> wp (fun a -> p (V a))
 
 type lex_t =
   | LexTop  : lex_t
   | LexCons : #a:Type -> a -> lex_t -> lex_t
 
-(* 'a * 'b *)
 type Tuple2 'a 'b =
   | MkTuple2: _1:'a
            -> _2:'b
            -> Tuple2 'a 'b
 
-(* 'a * 'b * 'c *)
 type Tuple3 'a 'b 'c =
   | MkTuple3: _1:'a
            -> _2:'b
            -> _3:'c
           -> Tuple3 'a 'b 'c
 
-(* 'a * 'b * 'c * 'd *)
 type Tuple4 'a 'b 'c 'd =
   | MkTuple4: _1:'a
            -> _2:'b
@@ -469,7 +440,6 @@ type Tuple4 'a 'b 'c 'd =
            -> _4:'d
            -> Tuple4 'a 'b 'c 'd
 
-(* 'a * 'b * 'c * 'd * 'e *)
 type Tuple5 'a 'b 'c 'd 'e =
   | MkTuple5: _1:'a
            -> _2:'b
@@ -478,7 +448,6 @@ type Tuple5 'a 'b 'c 'd 'e =
            -> _5:'e
            -> Tuple5 'a 'b 'c 'd 'e
 
-(* 'a * 'b * 'c * 'd * 'e * 'f *)
 type Tuple6 'a 'b 'c 'd 'e 'f =
   | MkTuple6: _1:'a
            -> _2:'b
@@ -489,7 +458,6 @@ type Tuple6 'a 'b 'c 'd 'e 'f =
            -> Tuple6 'a 'b 'c 'd 'e 'f
 
 
-(* 'a * 'b * 'c * 'd * 'e * 'f * 'g *)
 type Tuple7 'a 'b 'c 'd 'e 'f 'g =
   | MkTuple7: _1:'a
            -> _2:'b
@@ -500,7 +468,7 @@ type Tuple7 'a 'b 'c 'd 'e 'f 'g =
            -> _7:'g
            -> Tuple7 'a 'b 'c 'd 'e 'f 'g
 
-(* 'a * 'b * 'c * 'd * 'e * 'f * 'g * 'h *)
+
 type Tuple8 'a 'b 'c 'd 'e 'f 'g 'h =
   | MkTuple8: _1:'a
            -> _2:'b
@@ -512,73 +480,82 @@ type Tuple8 'a 'b 'c 'd 'e 'f 'g 'h =
            -> _8:'h
            -> Tuple8 'a 'b 'c 'd 'e 'f 'g 'h
 
-(* Concrete syntax (x:a & y:b x & c x y) *)
-type DTuple3 (a:Type)
-             (b:(a -> GTot Type))
-             (c:(x:a -> b x -> GTot Type)) =
-   | MkDTuple3:_1:a
-             -> _2:b _1
-             -> _3:c _1 _2
-             -> DTuple3 a b c
+type DTuple3: a:Type
+            -> b:(a -> Type)
+            -> c:(x:a -> b x -> Type)
+            -> Type =
+   | MkDTuple3: #a:Type
+            ->  #b:(a -> Type)
+            ->  #c:(x:a -> b x -> Type)
+            -> _1:a
+            -> _2:b _1
+            -> _3:c _1 _2
+            -> DTuple3 a b c
 
-(* Concrete syntax (x:a & y:b x & z:c x y & d x y z) *)
-type DTuple4 (a:Type)
-             (b:(x:a -> GTot Type))
-             (c:(x:a -> b x -> GTot Type))
-             (d:(x:a -> y:b x -> z:c x y -> GTot Type)) =
- | MkDTuple4:_1:a
+type DTuple4: a:Type
+           -> b:(x:a -> Type)
+           -> c:(x:a -> b x -> Type)
+           -> d:(x:a -> y:b x -> z:c x y -> Type)
+           -> Type =
+ | MkDTuple4: #a:Type
+           -> #b:(a -> Type)
+           -> #c:(x:a -> b x -> Type)
+           -> #d:(x:a -> y:b x -> z:c x y -> Type)
+           -> _1:a
            -> _2:b _1
            -> _3:c _1 _2
            -> _4:d _1 _2 _3
            -> DTuple4 a b c d
 
-let as_requires (#a:Type) (wp:pure_wp a)  = wp (fun x -> True)
-let as_ensures  (#a:Type) (wlp:pure_wp a) (x:a) = ~ (wlp (fun y -> (y=!=x)))
+
+type as_requires (#a:Type) (wp:PureWP a)  = wp (fun x -> True)
+type as_ensures  (#a:Type) (wlp:PureWP a) (x:a) = ~ (wlp (fun y -> ~(y=x)))
 
 val fst : ('a * 'b) -> Tot 'a
 let fst x = MkTuple2._1 x
 
+
 val snd : ('a * 'b) -> Tot 'b
 let snd x = MkTuple2._2 x
 
-val dfst : #a:Type -> #b:(a -> GTot Type) -> DTuple2 a b -> Tot a
-let dfst #a #b t = MkDTuple2._1 t
+val dfst : #a:Type -> #b:(a -> Type) -> DTuple2 a b -> Tot a
+let dfst t = MkDTuple2._1 t
 
-val dsnd : #a:Type -> #b:(a -> GTot Type) -> t:DTuple2 a b -> Tot (b (MkDTuple2._1 t))
-let dsnd #a #b t = MkDTuple2._2 t
+val dsnd : #a:Type -> #b:(a -> Type) -> t:(DTuple2 a b) -> Tot (b (MkDTuple2._1 t))
+let dsnd t = MkDTuple2._2 t
 
 type Let (#a:Type) (x:a) (body:(a -> Type)) = body x
-assume type InductionHyp : #a:Type -> a -> Type -> Type
+logic type InductionHyp : #a:Type -> a -> Type -> Type
 assume val by_induction_on: #a:Type -> #p:Type -> induction_on:a -> proving:p -> Lemma (ensures (InductionHyp induction_on p))
-assume type Using : #a:Type -> Type -> a -> Type
+logic type Using : #a:Type -> Type -> a -> Type
 assume val using: #a:Type -> #p:Type -> proving:p -> pat:a -> Lemma (ensures (Using p pat))
 assume val _assume : p:Type -> unit -> Pure unit (requires (True)) (ensures (fun x -> p))
 assume val admit   : #a:Type -> unit -> Admit a
 assume val magic   : #a:Type -> unit -> Tot a
+assume val unsafe_coerce  : #a:Type -> #b: Type -> a -> Tot b
 assume val admitP  : p:Type -> Pure unit True (fun x -> p)
 assume val _assert : p:Type -> unit -> Pure unit (requires $"assertion failed" p) (ensures (fun x -> True))
 assume val cut     : p:Type -> Pure unit (requires $"assertion failed" p) (fun x -> p)
-assume val qintro  : #a:Type -> #p:(a -> GTot Type) -> =f:(x:a -> Lemma (p x)) -> Lemma (forall (x:a). p x)
-assume val ghost_lemma: #a:Type -> #p:(a -> GTot Type) -> #q:(a -> unit -> GTot Type) -> =f:(x:a -> Ghost unit (p x) (q x)) -> Lemma (forall (x:a). p x ==> q x ())
+assume val qintro  : #a:Type -> #p:(a -> Type) -> =f:(x:a -> Lemma (p x)) -> Lemma (forall (x:a). p x)
+assume val ghost_lemma: #a:Type -> #p:(a -> Type) -> #q:(a -> unit -> Type) -> =f:(x:a -> Ghost unit (p x) (q x)) -> Lemma (forall (x:a). p x ==> q x ())
 assume val raise: exn -> Ex 'a       (* TODO: refine with the Exn monad *)
-val ignore: #a:Type -> a -> Tot unit
-let ignore #a x = ()
+val ignore: 'a -> Tot unit
+let ignore x = ()
 
 type nat = i:int{i >= 0}
 type pos = i:int{i > 0}
 type nonzero = i:int{i<>0}
 
-(*    For the moment we require not just that the divisor is non-zero, *)
-(*    but also that the dividend is natural. This works around a *)
-(*    mismatch between the semantics of integer division in SMT-LIB and *)
-(*    in F#/OCaml. For SMT-LIB ints the modulus is always positive (as in *)
-(*    math Euclidian division), while for F#/OCaml ints the modulus has *)
-(*    the same sign as the dividend. Our arbitrary precision ints don't *)
-(*    quite correspond to finite precision F#/OCaml ints though, but to *)
-(*    OCaml's big_ints (for which the modulus is always positive).  So *)
-(*    we'll need to return to this point anyway, when we discuss how to *)
-(*    soundly map F* ints to something in F#/OCaml.  *)
-
+(* For the moment we require not just that the divisor is non-zero,
+   but also that the dividend is natural. This works around a
+   mismatch between the semantics of integer division in SMT-LIB and
+   in F#/OCaml. For SMT-LIB ints the modulus is always positive (as in
+   math Euclidian division), while for F#/OCaml ints the modulus has
+   the same sign as the dividend. Our arbitrary precision ints don't
+   quite correspond to finite precision F#/OCaml ints though, but to
+   OCaml's big_ints (for which the modulus is always positive).  So
+   we'll need to return to this point anyway, when we discuss how to
+   soundly map F* ints to something in F#/OCaml. *)
 assume val op_Modulus            : int -> nonzero -> Tot int
 assume val op_Division           : nat -> nonzero -> Tot int
 
