lib/FStar.FunctionalExtensionality.fst
@@ -19,8 +19,10 @@ module FStar.FunctionalExtensionality
 
 type efun (a:Type) (b:Type) = a -> Tot b
 
-type FEq (#a:Type) (#b:Type) (f:efun a b) (g:efun a b) =
+opaque type FEq (#a:Type) (#b:Type) (f:efun a b) (g:efun a b) =
   (forall x.{:pattern (f x) \/ (g x)} f x = g x)
 
 assume Extensionality : forall (a:Type) (b:Type) (f: efun a b) (g: efun a b).
                         {:pattern FEq #a #b f g} FEq #a #b f g <==> f=g
+
+end
