lib/FStar.Squash.fst
@@ -1,47 +1,25 @@
-(* Interface for squash types; somehow inspired by:
-   Quotient Types: A Modular Approach. Aleksey Nogin, TPHOLs 2002.
-   http://www.nuprl.org/documents/Nogin/QuotientTypes_02.pdf
-*)
 module FStar.Squash
 
 (* This file shows that there is a natural model for some of the squash things;
+   DO NOT IMPORT THIS FILE; USE FStar.Squash.fsti and --admit_fsi FStar.Squash INSTEAD
  *)
 
-abstract type squash (t:Type) = t
+type squash (t:Type) = t
 
-abstract val give_proof : #p:Type -> squash p ->
-  Pure unit (requires True) (ensures (fun _ -> p))
+let return_squash x = x
 
-abstract val proof_irrelevance : p:Type -> x:squash p ->
-                                 y:squash p -> Tot (squash (x = y))
+let bind_squash x f = f x
 
-abstract val squash_double_arrow : #a:Type -> #p:(a -> Type) ->
-  =f:(squash (x:a -> Tot (squash (p x)))) -> Tot (squash (x:a -> Tot (p x)))
+let map_squash x f = f x
 
-(* This is a monad, but not an effect *)
+(* Inconsistent, see #355 *)
+assume val get_proof : p:Type ->
+  Pure (squash p) (requires p) (ensures (fun _ -> True))
 
-abstract val return_squash : #a:Type -> a -> Tot (squash a)
-
-abstract val bind_squash : #a:Type -> #b:Type -> squash a -> (a -> Tot (squash b)) ->
-  Tot (squash b)
-
-abstract val map_squash : #a:Type -> #b:Type -> squash a -> (a -> Tot b) ->
-  Tot (squash b)
-
-let return_squash #a x = x
-
-let bind_squash #a #b x f = f x
-
-let map_squash #a #b x f = f x
-
-let give_proof #p s = ()
-
-let squash_double_arrow #a #p f = f
+let give_proof (#p:Type) (s:squash p) = ()
 
 (* Inconsistent *)
 assume val proof_irrelevance : p:Type -> x:squash p ->
                                         y:squash p -> Tot (squash (x = y))
 
-(* Inconsistent, see #355 *)
-assume val get_proof : p:Type ->
-  Pure (squash p) (requires p) (ensures (fun _ -> True))
+let squash_double_arrow (#a:Type) (#p:a -> Type) f = f
