ulib/FStar.All.fst
@@ -1,0 +1,46 @@
+(*--build-config
+options:--admit_fsi FStar.Set;
+other-files: FStar.Set.fsi FStar.Heap.fst FStar.ST.fst;
+--*)
+(*
+   Copyright 2008-2014 Nikhil Swamy and Microsoft Research
+
+   Licensed under the Apache License, Version 2.0 (the "License");
+   you may not use this file except in compliance with the License.
+   You may obtain a copy of the License at
+
+       http://www.apache.org/licenses/LICENSE-2.0
+
+   Unless required by applicable law or agreed to in writing, software
+   distributed under the License is distributed on an "AS IS" BASIS,
+   WITHOUT WARRANTIES OR CONDITIONS OF ANY KIND, either express or implied.
+   See the License for the specific language governing permissions and
+   limitations under the License.
+*)
+module FStar.All
+open FStar.Heap
+open FStar.ST
+
+let all_pre = all_pre_h heap
+let all_post (a:Type) = all_post_h heap a
+let all_wp (a:Type) = all_wp_h heap a
+new_effect ALL = ALL_h heap
+
+inline let lift_state_all (a:Type) (wp:st_wp a) (p:all_post a) =  wp (fun a -> p (V a))
+sub_effect STATE ~> ALL = lift_state_all
+
+inline let lift_exn_all (a:Type) (wp:ex_wp a)   (p:all_post a) (h:heap) = wp (fun ra -> p ra h)
+sub_effect EXN   ~> ALL = lift_exn_all
+
+effect All (a:Type) (pre:all_pre) (post: (heap -> Tot (all_post a))) =
+       ALL a
+           (fun (p:all_post a) (h:heap) -> pre h /\ (forall ra h1. post h ra h1 ==> p ra h1)) (* WP  *)
+           (fun (p:all_post a) (h:heap) -> forall ra h1. (pre h /\ post h ra h1) ==> p ra h1) (* WLP *)
+default effect ML (a:Type) =
+  ALL a (all_null_wp heap a) (all_null_wp heap a)
+
+assume val pipe_right: 'a -> ('a -> 'b) -> 'b
+assume val pipe_left: ('a -> 'b) -> 'a -> 'b
+assume val failwith: string -> All 'a (fun h -> True) (fun h a h' -> is_Err a /\ h==h')
+assume val exit: int -> 'a
+assume val try_with: (unit -> 'a) -> (exn -> 'a) -> 'a
