ulib/FStar.Option.fst
@@ -1,0 +1,25 @@
+(*--build-config
+  options: --admit_fsi FStar.Set;
+  other-files: FStar.Set.fsi FStar.Heap.fst FStar.ST.fst FStar.All.fst
+  --*)
+(*
+   Copyright 2008-2014 Nikhil Swamy and Microsoft Research
+
+   Licensed under the Apache License, Version 2.0 (the "License");
+   you may not use this file except in compliance with the License.
+   You may obtain a copy of the License at
+
+       http://www.apache.org/licenses/LICENSE-2.0
+
+   Unless required by applicable law or agreed to in writing, software
+   distributed under the License is distributed on an "AS IS" BASIS,
+   WITHOUT WARRANTIES OR CONDITIONS OF ANY KIND, either express or implied.
+   See the License for the specific language governing permissions and
+   limitations under the License.
+*)
+module FStar.Option
+
+assume val isNone: option 'a -> bool
+assume val isSome: option 'a -> bool
+assume val map: ('a -> 'b) -> option 'a -> option 'b
+assume val get: option 'a -> 'a 
