ulib/FStar.PredicateExtensionality.fst
@@ -1,0 +1,16 @@
+
+(* CH: because of the stratified nature of F* this variant of
+   extensionality doesn't seem to follow from functional and
+   propositional extensionality; does it? *)
+
+module FStar.PredicateExtensionality
+#set-options "--max_fuel 0 --initial_fuel 0 --initial_ifuel 0 --max_ifuel 0"
+
+let predicate (a:Type) = a -> Type
+
+let peq (#a:Type) (p1:predicate a) (p2:predicate a) = forall x. p1 x <==> p2 x
+
+assume val predicateExtensionality : a:Type -> p1:predicate a -> p2:predicate a ->
+  Lemma (requires True)
+	(ensures (peq #a p1 p2 <==> p1==p2))
+	[SMTPat (peq #a p1 p2)]
